src/SimplExpr.v
@@ -30,36 +30,6 @@ Local Open Scope list_scope.
 
 (* (** State and error monad for generating fresh identifiers. *) *)
 
-(* Record generator : Type := mkgenerator { *)
-(*   gen_next: ident; *)
-(*   gen_trail: list (ident * type) *)
-(* }. *)
-
-(* Inductive result (A: Type) (g: generator) : Type := *)
-(*   | Err: Errors.errmsg -> result A g *)
-(*   | Res: A -> forall (g': generator), Ple (gen_next g) (gen_next g') -> result A g. *)
-
-(* Arguments Err [A g]. *)
-(* Arguments Res [A g]. *)
-
-(* Definition mon (A: Type) := forall (g: generator), result A g. *)
-
-(* Definition ret {A: Type} (x: A) : mon A := *)
-(*   fun g => Res x g (Ple_refl (gen_next g)). *)
-
-(* Definition error {A: Type} (msg: Errors.errmsg) : mon A := *)
-(*   fun g => Err msg. *)
-
-(* Definition bind {A B: Type} (x: mon A) (f: A -> mon B) : mon B := *)
-(*   fun g => *)
-(*     match x g with *)
-(*       | Err msg => Err msg *)
-(*       | Res a g' i => *)
-(*           match f a g' with *)
-(*           | Err msg => Err msg *)
-(*           | Res b g'' i' => Res b g'' (Ple_trans _ _ _ i i') *)
-(*       end *)
-(*     end. *)
 Import gensym.
 Definition bind2 {A B C: Type} (x: mon (A * B)) (f: A -> B -> mon C) : mon C :=
   bind x (fun p => f (fst p) (snd p)).
