src/SimplExprproof.v
@@ -1,0 +1,2066 @@
+(* *********************************************************************)
+(*                                                                     *)
+(*              The Compcert verified compiler                         *)
+(*                                                                     *)
+(*          Xavier Leroy, INRIA Paris-Rocquencourt                     *)
+(*                                                                     *)
+(*  Copyright Institut National de Recherche en Informatique et en     *)
+(*  Automatique.  All rights reserved.  This file is distributed       *)
+(*  under the terms of the INRIA Non-Commercial License Agreement.     *)
+(*                                                                     *)
+(* *********************************************************************)
+
+(** Correctness proof for expression simplification. *)
+
+Require Import FunInd.
+Require Import Coqlib (* Maps *) Errors Integers.
+Require Import AST Linking.
+Require Import Values Memory Events Globalenvs Smallstep.
+Require Import Ctypes Cop Csyntax Csem Cstrategy Clight.
+Import Maps.PTree.
+Require Import MoSel SimplExpr SimplExprspec.
+
+Local Open Scope gensym_monad_scope.
+Notation "a ! b" := (get b a) (at level 1).
+(** ** Relational specification of the translation. *)
+
+Definition match_prog (p: Csyntax.program) (tp: Clight.program) :=
+    match_program (fun ctx f tf => tr_fundef f tf) eq p tp
+ /\ prog_types tp = prog_types p.
+
+Lemma transf_program_match:
+  forall p tp, transl_program p = OK tp -> match_prog p tp.
+Proof.
+  unfold transl_program; intros. monadInv H. split; auto.
+  unfold program_of_program; simpl. destruct x; simpl.
+  eapply match_transform_partial_program_contextual. eexact EQ. 
+  intros. apply transl_fundef_spec; auto. 
+Qed.
+
+(** ** Semantic preservation *)
+
+Section PRESERVATION.
+
+Variable prog: Csyntax.program.
+Variable tprog: Clight.program.
+Hypothesis TRANSL: match_prog prog tprog.
+
+Let ge := Csem.globalenv prog.
+Let tge := Clight.globalenv tprog.
+
+(** Invariance properties. *)
+
+Lemma comp_env_preserved:
+  Clight.genv_cenv tge = Csem.genv_cenv ge.
+Proof.
+  simpl. destruct TRANSL. generalize (prog_comp_env_eq tprog) (prog_comp_env_eq prog). 
+  congruence.
+Qed.
+
+Lemma symbols_preserved:
+  forall (s: ident), Genv.find_symbol tge s = Genv.find_symbol ge s.
+Proof (Genv.find_symbol_match (proj1 TRANSL)).
+
+Lemma senv_preserved:
+  Senv.equiv ge tge.
+Proof (Genv.senv_match (proj1 TRANSL)).
+
+Lemma function_ptr_translated:
+  forall b f,
+  Genv.find_funct_ptr ge b = Some f ->
+  exists tf,
+  Genv.find_funct_ptr tge b = Some tf /\ tr_fundef f tf.
+Proof.
+  intros.
+  edestruct (Genv.find_funct_ptr_match (proj1 TRANSL)) as (ctx & tf & A & B & C); eauto.
+Qed.
+
+Lemma functions_translated:
+  forall v f,
+  Genv.find_funct ge v = Some f ->
+  exists tf,
+  Genv.find_funct tge v = Some tf /\ tr_fundef f tf.
+Proof.
+  intros.
+  edestruct (Genv.find_funct_match (proj1 TRANSL)) as (ctx & tf & A & B & C); eauto.
+Qed.
+
+Lemma type_of_fundef_preserved:
+  forall f tf, tr_fundef f tf ->
+  type_of_fundef tf = Csyntax.type_of_fundef f.
+Proof.
+  intros. inv H.
+  inv H0; simpl. unfold type_of_function, Csyntax.type_of_function. congruence.
+  auto.
+Qed.
+
+Lemma function_return_preserved:
+  forall f tf, tr_function f tf ->
+  fn_return tf = Csyntax.fn_return f.
+Proof.
+  intros. inv H; auto.
+Qed.
+
+(** Properties of smart constructors. *)
+
+Lemma eval_Ederef':
+  forall ge e le m a t l ofs,
+  eval_expr ge e le m a (Vptr l ofs) ->
+  eval_lvalue ge e le m (Ederef' a t) l ofs.
+Proof.
+  intros. unfold Ederef'; destruct a; auto using eval_Ederef.
+  destruct (type_eq t0 (typeof a)); auto using eval_Ederef.
+  inv H.
+- auto. 
+- inv H0.
+Qed.
+
+Lemma typeof_Ederef':
+  forall a t, typeof (Ederef' a t) = t.
+Proof.
+  unfold Ederef'; intros; destruct a; auto. destruct (type_eq t0 (typeof a)); auto. 
+Qed.
+
+Lemma eval_Eaddrof':
+  forall ge e le m a t l ofs,
+  eval_lvalue ge e le m a l ofs ->
+  eval_expr ge e le m (Eaddrof' a t) (Vptr l ofs).
+Proof.
+  intros. unfold Eaddrof'; destruct a; auto using eval_Eaddrof.
+  destruct (type_eq t0 (typeof a)); auto using eval_Eaddrof.
+  inv H; auto.
+Qed.
+
+Lemma typeof_Eaddrof':
+  forall a t, typeof (Eaddrof' a t) = t.
+Proof.
+  unfold Eaddrof'; intros; destruct a; auto. destruct (type_eq t0 (typeof a)); auto. 
+Qed.
+
+(** Translation of simple expressions. *)
+
+Lemma pair_equal_spec :
+  forall (A B : Type) (a1 a2 : A) (b1 b2 : B),
+    (a1, b1) = (a2, b2) <-> a1 = a2 /\ b1 = b2.
+Proof.
+  intros. split; intro H; inversion H; subst; eauto.
+Qed.
+
+Import adequacy.
+
+Lemma tr_simple_nil:
+  (forall r dst sl le a, tr_expr le dst r (sl,a) -∗
+   ⌜ dst = For_val \/ dst = For_effects ⌝ -∗ ⌜ simple r = true ⌝ -∗ ⌜sl = nil ⌝)
+/\(forall rl le sl al, tr_exprlist le rl (sl,al) -∗
+   ⌜ simplelist rl = true ⌝ -∗ ⌜ sl = nil ⌝).
+Proof.
+  assert (A: forall dst a, dst = For_val \/ dst = For_effects -> final dst a = nil).
+  intros. destruct H; subst dst; auto.
+  apply tr_expr_exprlist; intros; simpl in *; try discriminate; auto.
+  - destruct dst.
+    + iIntros "[% [% %]]". iPureIntro. intros; auto.
+    + iIntros. iPureIntro. intros; auto.
+    + iIntros "[% [% %]]". iPureIntro. intros. destruct H2; discriminate.
+  - iIntros "[_ %]". iPureIntro. intros. inversion H. destruct dst; auto.
+  - iIntros "HA". iDestruct "HA" as (sla2) "[HA [HB %]]".
+    rewrite (surjective_pairing sla2). iIntros.
+    iDestruct (H with "[HA]") as "HC". iApply "HA".
+    destruct dst.
+    + iDestruct ("HC" $! a0 a1) as "HA". simpl in *. inversion H0. rewrite app_nil_r. iApply "HA". 
+    + iDestruct ("HC" with "[]") as "HA"; eauto. inversion H0. rewrite app_nil_r.
+      iApply ("HA" $! a1).
+    + destruct a0; discriminate.
+  - iIntros "HA % %". iDestruct "HA" as (sla2 sl3) "[HA [HB [HC %]]]".
+    rewrite (surjective_pairing sla2).
+    iDestruct (H with "HA") as "HD".
+    apply andb_true_iff in a1 as (P0&P1).
+    unfold tr_rvalof. apply negb_true_iff in P1. rewrite P1.
+    iDestruct "HB" as "%". inversion H1; subst. destruct dst; simpl in *; try rewrite app_nil_r.
+    + iApply ("HD" $! a0 P0).
+    + iApply "HD"; eauto.
+    + destruct a0; discriminate.
+  - iIntros "HA % %". iDestruct "HA" as (sla2) "[HA [HB %]]".
+    rewrite (surjective_pairing sla2).
+    iDestruct (H with "HA") as "HD".
+    inversion H0.
+    destruct dst; simpl in *; try (rewrite app_nil_r; iApply "HD";eauto); destruct a0; discriminate.
+  - iIntros "HA % %". iDestruct "HA" as (sla2) "[HA [HB %]]".
+    rewrite (surjective_pairing sla2).
+    iDestruct (H with "HA") as "HD".
+    inversion H0.
+    destruct dst; simpl in *; try (rewrite app_nil_r; iApply "HD";eauto); destruct a0; discriminate.
+  - iIntros "HA % %". iDestruct "HA" as (sla2) "[HA [HB %]]".
+    rewrite (surjective_pairing sla2).
+    iDestruct (H with "HA") as "HD".
+    inversion H0.
+    destruct dst; simpl in *; try (rewrite app_nil_r; iApply "HD";eauto); destruct a0; discriminate.
+  - iIntros "HA % %". iDestruct "HA" as (sla2 sl3) "[HA [HB [HC %]]]".
+    rewrite (surjective_pairing sla2).
+    iDestruct (H with "HA") as "HD".
+    rewrite (surjective_pairing sl3).
+    iDestruct (H0 with "HB") as "HB".
+    apply andb_true_iff in a1 as (P0&P1).
+    inversion H1.
+    iDestruct ("HD" with "[]") as "%"; eauto.
+    iDestruct ("HB" with "[]") as "%"; eauto.
+    iPureIntro. rewrite (H2 P0). rewrite (H5 P1).
+    destruct a0; subst; auto.
+  - iIntros "HA % %". iDestruct "HA" as (sla2) "[HA [HB %]]".
+    rewrite (surjective_pairing sla2).
+    iDestruct (H with "HA") as "HD".
+    inversion H0.
+    destruct dst; simpl in *; try (rewrite app_nil_r; iApply "HD";eauto); destruct a0; discriminate.
+  - iIntros "[HA %] % %". inversion H.
+    destruct dst; eauto.
+  - iIntros "[HA %] % %". inversion H.
+    destruct dst; eauto.
+  - iIntros "% %". inversion a; eauto.
+  - iIntros "HA %". iDestruct "HA" as (sla2 slal3) "[HA [HB %]]".
+    rewrite (surjective_pairing sla2).
+    iDestruct (H with "[HA]") as "HC". iApply "HA".
+    rewrite (surjective_pairing slal3).
+    iDestruct (H0 with "[HB]") as "HA". iApply "HB".
+    iDestruct ("HC" with "[]") as "%"; eauto.
+    apply andb_true_iff in a as (P0&P1).
+    iDestruct ("HA" with "[]") as "%"; eauto.
+    iPureIntro. inversion H1. rewrite (H2 P0). rewrite H3. eauto.
+Qed.
+
+Lemma tr_simple_expr_nil:
+  (forall r dst sl le a, tr_expr le dst r (sl,a) -∗
+   ⌜ dst = For_val \/ dst = For_effects ⌝ -∗ ⌜ simple r = true ⌝ -∗ ⌜sl = nil ⌝).
+Proof (proj1 tr_simple_nil).
+
+Lemma tr_simple_exprlist_nil:
+  (forall rl le sl al, tr_exprlist le rl (sl,al) -∗
+   ⌜ simplelist rl = true ⌝ -∗ ⌜ sl = nil ⌝).
+Proof (proj2 tr_simple_nil).
+
+(** Translation of [deref_loc] and [assign_loc] operations. *)
+
+Remark deref_loc_translated:
+  forall ty m b ofs t v,
+  Csem.deref_loc ge ty m b ofs t v ->
+  match chunk_for_volatile_type ty with
+  | None => t = E0 /\ Clight.deref_loc ty m b ofs v
+  | Some chunk => volatile_load tge chunk m b ofs t v
+  end.
+Proof.
+  intros. unfold chunk_for_volatile_type. inv H.
+  (* By_value, not volatile *)
+  rewrite H1. split; auto. eapply deref_loc_value; eauto.
+  (* By_value, volatile *)
+  rewrite H0; rewrite H1. eapply volatile_load_preserved with (ge1 := ge); auto. apply senv_preserved.
+  (* By reference *)
+  rewrite H0. destruct (type_is_volatile ty); split; auto; eapply deref_loc_reference; eauto.
+  (* By copy *)
+  rewrite H0. destruct (type_is_volatile ty); split; auto; eapply deref_loc_copy; eauto.
+Qed.
+
+Remark assign_loc_translated:
+  forall ty m b ofs v t m',
+  Csem.assign_loc ge ty m b ofs v t m' ->
+  match chunk_for_volatile_type ty with
+  | None => t = E0 /\ Clight.assign_loc tge ty m b ofs v m'
+  | Some chunk => volatile_store tge chunk m b ofs v t m'
+  end.
+Proof.
+  intros. unfold chunk_for_volatile_type. inv H.
+  (* By_value, not volatile *)
+  rewrite H1. split; auto. eapply assign_loc_value; eauto.
+  (* By_value, volatile *)
+  rewrite H0; rewrite H1. eapply volatile_store_preserved with (ge1 := ge); auto. apply senv_preserved.
+  (* By copy *)
+  rewrite H0. rewrite <- comp_env_preserved in *.
+  destruct (type_is_volatile ty); split; auto; eapply assign_loc_copy; eauto.
+Qed.
+
+(** Evaluation of simple expressions and of their translation *)
+Import adequacy.
+Lemma tr_simple:
+ forall e m,
+ (forall r v,
+  eval_simple_rvalue ge e m r v ->
+  forall le dst sl a,
+  (tr_expr le dst r (sl,a)) -∗
+  match dst with
+  | For_val => ⌜ sl = nil /\ Csyntax.typeof r = typeof a /\ eval_expr tge e le m a v ⌝
+  | For_effects => ⌜ sl = nil ⌝
+  | For_set sd =>
+      ∃ b, ⌜ sl = do_set sd b
+             /\ Csyntax.typeof r = typeof b
+             /\ eval_expr tge e le m b v ⌝
+  end)
+/\
+ (forall l b ofs,
+  eval_simple_lvalue ge e m l b ofs ->
+  forall le sl a, tr_expr le For_val l (sl,a) -∗                                               
+  ⌜ sl = nil /\ Csyntax.typeof l = typeof a /\ eval_lvalue tge e le m a b ofs ⌝).
+Proof.
+Opaque makeif.
+intros e m.
+apply (eval_simple_rvalue_lvalue_ind ge e m); intros; simpl.
+(* value *)
+- destruct dst; simpl in *; iIntros "%".
+  + destruct a0 as (P0&P1&P2). iPureIntro. repeat split; auto. 
+  + iPureIntro. assumption.
+  + iExists a. destruct a0 as (P0&P1&P2). iPureIntro. split; auto.
+(* rvalof *)
+- destruct dst; subst; simpl in *.
+  + iIntros "HA". iDestruct "HA" as (sla2 sl3) "[HA [HB [_ %]]]".
+    rewrite (surjective_pairing sla2).
+    iDestruct (H0 with "HA") as "[% [% %]]".
+    unfold tr_rvalof. rewrite H2. iDestruct "HB" as "%". inversion H7; subst.
+    iPureIntro. repeat split; auto. do 2 rewrite app_nil_r. apply H4.
+    eapply eval_Elvalue; eauto.
+    exploit deref_loc_translated; eauto. unfold chunk_for_volatile_type; rewrite H2.
+    intros (P0&P1). rewrite <- H5. assumption.
+  + iIntros "HA". iDestruct "HA" as (sla2 sl3) "[HA [HB [_ %]]]".
+    rewrite (surjective_pairing sla2).
+    iDestruct (H0 with "HA") as "[% [% %]]".
+    unfold tr_rvalof. rewrite H2. iDestruct "HB" as "%". inversion H7; subst.
+    iPureIntro. do 2 rewrite app_nil_r. apply H4.
+  + iIntros "HA". iDestruct "HA" as (sla2 sl3) "[HA [HB [_ %]]]". iExists a.
+    rewrite (surjective_pairing sla2).
+    iDestruct (H0 with "HA") as "[% [% %]]".
+    unfold tr_rvalof. rewrite H2. iDestruct "HB" as "%". inversion H7; subst.
+    iPureIntro. repeat split; auto. rewrite H4. do 2 rewrite app_nil_l. reflexivity.
+    eapply eval_Elvalue; eauto.
+    exploit deref_loc_translated; eauto. unfold chunk_for_volatile_type; rewrite H2.
+    intros (P0&P1). rewrite <- H5. apply P1.
+- iIntros "HA". iDestruct "HA" as (sla2) "[HA [HB %]]". rewrite (surjective_pairing sla2).
+  iDestruct (H0 with "HA") as "[% [% %]]". inversion H1.
+  destruct dst; simpl in *; subst.
+  + iPureIntro. repeat split; auto.
+    * rewrite app_nil_r. apply H2.
+    * rewrite (typeof_Eaddrof' sla2.2 ty). reflexivity.
+    * apply eval_Eaddrof'; auto.
+  + iPureIntro. rewrite app_nil_r. apply H2.
+  + iExists (Eaddrof' sla2.2 ty). iPureIntro. repeat split.
+    * rewrite H2. rewrite app_nil_l. reflexivity.
+    * rewrite (typeof_Eaddrof' sla2.2 ty). reflexivity.
+    * apply eval_Eaddrof'; auto.
+- iIntros "HA". iDestruct "HA" as (sla2) "[HA [HB %]]". rewrite (surjective_pairing sla2).
+  iDestruct (H0 with "HA") as "[% [% %]]". inversion H2.
+  destruct dst; simpl in *; subst.
+  + iPureIntro. repeat split; auto.
+    * rewrite app_nil_r. apply H3.
+    * rewrite H4 in H1. econstructor; eauto.
+  + iPureIntro. rewrite app_nil_r. apply H3.
+  + iExists (Eunop op0 sla2.2 ty). iPureIntro. repeat split.
+    * rewrite H3. rewrite app_nil_l. reflexivity.
+    * rewrite H4 in H1. econstructor; eauto.
+- iIntros "HA". iDestruct "HA" as (sla2 sla3) "[HA [HB [HC %]]]". rewrite (surjective_pairing sla2).
+  iDestruct (H0 with "HA") as "[% [% %]]". rewrite (surjective_pairing sla3).
+  iDestruct (H2 with "HB") as "[% [% %]]". inversion H4.
+  destruct dst; simpl in *; subst; rewrite H5 H8; try iExists (Ebinop op0 sla2.2 sla3.2 ty);
+    do 2 rewrite app_nil_l; iPureIntro; repeat split; auto; econstructor; eauto; rewrite <- H6;
+      auto; rewrite <- H9; rewrite comp_env_preserved; apply H3.
+- iIntros "HA". iDestruct "HA" as (sla2)  "[HA [HB %]]". rewrite (surjective_pairing sla2).
+  iDestruct (H0 with "HA") as "[% [% %]]". inversion H2.
+  destruct dst; simpl in *; subst; rewrite H3; try iExists (Ecast sla2.2 ty); iPureIntro;
+    rewrite app_nil_l; repeat split; auto; econstructor; eauto; rewrite <- H4; auto.
+- iIntros "[HA %]". inversion H.
+  destruct dst; simpl in *; subst; try iExists (Esizeof ty1 ty); iPureIntro; repeat split; eauto;
+    pose (P := comp_env_preserved); simpl in P; rewrite <- P; apply eval_Esizeof.
+- iIntros "[HA %]". inversion H.
+  destruct dst; simpl in *; subst; try iExists (Ealignof ty1 ty); iPureIntro; repeat split; eauto;
+    pose (P := comp_env_preserved); simpl in P; rewrite <- P; constructor.
+- iIntros. contradiction a0.
+- iIntros "[_ %]". inversion H0. iPureIntro. repeat split; auto. constructor. apply H.
+- iIntros "[_ %]". inversion H1. iPureIntro. repeat split; auto.
+  apply eval_Evar_global; auto.
+  rewrite symbols_preserved; auto.
+- iIntros "HA". iDestruct "HA" as (sla2)  "[HA [HB %]]". rewrite (surjective_pairing sla2).
+  iDestruct (H0 with "HA") as "[% [% %]]". inversion H1. iPureIntro. subst. repeat split.
+  rewrite app_nil_r. apply H2. rewrite typeof_Ederef'; auto. apply eval_Ederef'; auto. 
+- iIntros "HA". iDestruct "HA" as (sla2)  "[HA [HB %]]". rewrite (surjective_pairing sla2).
+  iDestruct (H0 with "HA") as "[% [% %]]". inversion H4. subst. iPureIntro. repeat split.
+  rewrite app_nil_r. apply H5. rewrite <- comp_env_preserved in *. rewrite H6 in H1.
+  eapply eval_Efield_struct; eauto.
+- iIntros "HA". iDestruct "HA" as (sla2)  "[HA [HB %]]". rewrite (surjective_pairing sla2).
+  iDestruct (H0 with "HA") as "[% [% %]]". inversion H3. subst. iPureIntro. repeat split.
+  rewrite app_nil_r. apply H4. rewrite <- comp_env_preserved in *. rewrite H5 in H1.
+  eapply eval_Efield_union; eauto.
+Qed.
+   
+Lemma tr_simple_rvalue:
+  forall e m r v,
+    eval_simple_rvalue ge e m r v ->
+  forall le dst sl a,
+  (tr_expr le dst r (sl,a)) -∗
+  match dst with
+  | For_val => ⌜ sl = nil /\ Csyntax.typeof r = typeof a /\ eval_expr tge e le m a v ⌝
+  | For_effects => ⌜ sl = nil ⌝
+  | For_set sd =>
+      ∃ b, ⌜ sl = do_set sd b
+             /\ Csyntax.typeof r = typeof b
+             /\ eval_expr tge e le m b v ⌝
+  end.
+Proof.
+  intros e m. exact (proj1 (tr_simple e m)).
+Qed.
+
+Lemma tr_simple_lvalue:
+  forall e m l b ofs,
+  eval_simple_lvalue ge e m l b ofs ->
+  forall le sl a, tr_expr le For_val l (sl,a) -∗                                               
+  ⌜ sl = nil /\ Csyntax.typeof l = typeof a /\ eval_lvalue tge e le m a b ofs ⌝.
+Proof.
+  intros e m. exact (proj2 (tr_simple e m)).
+Qed.
+
+Lemma tr_simple_exprlist:
+  forall le rl sl al,
+  tr_exprlist le rl (sl,al) -∗
+  ∀ e m tyl vl,
+  ⌜ eval_simple_list ge e m rl tyl vl ⌝ -∗
+  ⌜ sl = nil /\ eval_exprlist tge e le m al tyl vl ⌝.
+Proof.
+  induction rl.
+  - iIntros. inversion a.
+    iPureIntro. repeat split; eauto. inversion a0. constructor.
+  - simpl. iIntros (? ?) "HA". iIntros (? ? ? ?) "%". iDestruct "HA" as (sla2 slal3) "[HA [HB %]]".
+    rewrite (surjective_pairing slal3).
+    iDestruct (IHrl with "HB") as "HC".
+    inversion a3. subst.
+    iDestruct ("HC" with "[]") as "[% %]"; eauto.
+    epose (P := tr_simple_rvalue _ _ _ _ H2).
+    rewrite (surjective_pairing sla2).
+    iDestruct (P with "HA") as "[% [% %]]".
+    iPureIntro. inversion H. subst. split.
+    + rewrite H4 H0; auto.
+    + econstructor; eauto. rewrite <- H5. eauto.
+Qed.
+
+(** Commutation between the translation of expressions and left contexts. *)
+
+Lemma typeof_context:
+  forall k1 k2 C, leftcontext k1 k2 C ->
+  forall e1 e2, Csyntax.typeof e1 = Csyntax.typeof e2 ->
+  Csyntax.typeof (C e1) = Csyntax.typeof (C e2).
+Proof.
+  induction 1; intros; auto.
+Qed.
+
+Scheme leftcontext_ind2 := Minimality for leftcontext Sort Prop
+  with leftcontextlist_ind2 := Minimality for leftcontextlist Sort Prop.
+Combined Scheme leftcontext_leftcontextlist_ind from leftcontext_ind2, leftcontextlist_ind2.
+Notation "\s l" := (∃ t, l ↦ t) (at level 10).
+Lemma tr_expr_leftcontext_rec:
+ (
+  forall from to C, leftcontext from to C ->
+  forall le e dst sl a,
+  tr_expr le dst (C e) (sl,a)-∗
+  ∃ dst' sl1 sl2 a',
+  tr_expr le dst' e (sl1,a')  ∗ ⌜ sl = sl1 ++ sl2 ⌝
+  ∗ (∀ le' e' sl3,
+        tr_expr le' dst' e' (sl3,a') -∗
+        (∀ id, (\s id -∗ False) -∗ ⌜ le'!id = le!id ⌝) -∗
+        \⌜ Csyntax.typeof e' = Csyntax.typeof e ⌝ -∗
+        tr_expr le' dst (C e') ((sl3 ++ sl2),a))
+ ) /\ (
+  forall from C, leftcontextlist from C ->
+  forall le e sl a,
+  tr_exprlist le (C e) (sl,a) -∗
+  ∃ dst' sl1 sl2 a',
+  tr_expr le dst' e (sl1,a')
+  ∗ ⌜sl = sl1 ++ sl2⌝
+  ∗ (∀ le' e' sl3,
+        tr_expr le' dst' e' (sl3,a') -∗
+        (∀ id, (\s id -∗ False) -∗ ⌜ le'!id = le!id⌝) -∗
+        \⌜ Csyntax.typeof e' = Csyntax.typeof e ⌝ -∗
+        tr_exprlist le' (C e') ((sl3 ++ sl2),a))
+).
+Proof.
+  Admitted.
+
+Theorem tr_expr_leftcontext:
+  forall C le r dst sl a,
+  leftcontext RV RV C ->
+  tr_expr le dst (C r) (sl,a) -∗
+  ∃ dst' sl1 sl2 a',
+  tr_expr le dst' r (sl1,a')
+  ∗ ⌜ sl = sl1 ++ sl2 ⌝
+  ∗ (∀ le' r' sl3,
+        tr_expr le' dst' r' (sl3,a') -∗
+        (∀ id, (\s id -∗ False) -∗ ⌜ le'!id = le!id ⌝) -∗
+        \⌜ Csyntax.typeof r' = Csyntax.typeof r ⌝ -∗
+        tr_expr le' dst (C r') ((sl3 ++ sl2),a)).
+Proof.
+  intros. eapply (proj1 tr_expr_leftcontext_rec); eauto.
+Qed.
+
+Theorem tr_top_leftcontext:
+  forall e le m dst rtop sl a,
+  tr_top tge e le m dst rtop (sl,a) -∗
+  ∀ r C,
+  ⌜ rtop = C r ⌝ -∗
+  ⌜ leftcontext RV RV C ⌝ -∗
+  ∃ dst' sl1 sl2 a',
+  tr_top tge e le m dst' r (sl1,a')
+  ∗ ⌜ sl = sl1 ++ sl2 ⌝
+  ∗ (∀ le' m' r' sl3,
+        tr_expr le' dst' r' (sl3,a') -∗
+        (∀ id, (\s id -∗ False) -∗ ⌜le'!id = le!id ⌝) -∗
+        ⌜ Csyntax.typeof r' = Csyntax.typeof r ⌝ -∗
+        tr_top tge e le' m' dst (C r') ((sl3 ++ sl2),a)).
+Proof.
+Admitted.
+
+(** Semantics of smart constructors *)
+
+Remark sem_cast_deterministic:
+  forall v ty ty' m1 v1 m2 v2,
+  sem_cast v ty ty' m1 = Some v1 ->
+  sem_cast v ty ty' m2 = Some v2 ->
+  v1 = v2.
+Proof.
+  unfold sem_cast; intros. destruct (classify_cast ty ty'); try congruence.
+- destruct v; try congruence.
+  destruct Archi.ptr64; try discriminate.
+  destruct (Mem.weak_valid_pointer m1 b (Ptrofs.unsigned i)); inv H.
+  destruct (Mem.weak_valid_pointer m2 b (Ptrofs.unsigned i)); inv H0.
+  auto.
+- destruct v; try congruence. 
+  destruct (negb Archi.ptr64); try discriminate.
+  destruct (Mem.weak_valid_pointer m1 b (Ptrofs.unsigned i)); inv H.
+  destruct (Mem.weak_valid_pointer m2 b (Ptrofs.unsigned i)); inv H0.
+  auto.
+Qed.
+
+Lemma eval_simpl_expr_sound:
+  forall e le m a v, eval_expr tge e le m a v ->
+  match eval_simpl_expr a with Some v' => v' = v | None => True end.
+Proof.
+  induction 1; simpl; auto.
+  destruct (eval_simpl_expr a); auto. subst.
+  destruct (sem_cast v1 (typeof a) ty Mem.empty) as [v'|] eqn:C; auto.
+  eapply sem_cast_deterministic; eauto.
+  inv H; simpl; auto.
+Qed.
+
+Lemma static_bool_val_sound:
+  forall v t m b, bool_val v t Mem.empty = Some b -> bool_val v t m = Some b.
+Proof.
+  assert (A: forall b ofs, Mem.weak_valid_pointer Mem.empty b ofs = false).
+  { unfold Mem.weak_valid_pointer, Mem.valid_pointer, proj_sumbool; intros.
+    rewrite ! pred_dec_false; auto; apply Mem.perm_empty. }  
+  intros until b; unfold bool_val.
+  destruct (classify_bool t0); destruct v; destruct Archi.ptr64 eqn:SF; auto.
+- rewrite A; congruence.
+- simpl; rewrite A; congruence.
+Qed.
+
+Lemma step_makeif:
+  forall f a s1 s2 k e le m v1 b,
+  eval_expr tge e le m a v1 ->
+  bool_val v1 (typeof a) m = Some b ->
+  star step1 tge (State f (makeif a s1 s2) k e le m)
+             E0 (State f (if b then s1 else s2) k e le m).
+Proof.
+  intros. functional induction (makeif a s1 s2).
+- exploit eval_simpl_expr_sound; eauto. rewrite e0. intro EQ; subst v.
+  assert (bool_val v1 (typeof a) m = Some true) by (apply static_bool_val_sound; auto).
+  replace b with true by congruence. constructor.
+- exploit eval_simpl_expr_sound; eauto. rewrite e0. intro EQ; subst v.
+  assert (bool_val v1 (typeof a) m = Some false) by (apply static_bool_val_sound; auto).
+  replace b with false by congruence. constructor.
+- apply star_one. eapply step_ifthenelse; eauto.
+- apply star_one. eapply step_ifthenelse; eauto.
+Qed.
+
+Lemma step_make_set:
+  forall id a ty m b ofs t v e le f k,
+  Csem.deref_loc ge ty m b ofs t v ->
+  eval_lvalue tge e le m a b ofs ->
+  typeof a = ty ->
+  step1 tge (State f (make_set id a) k e le m)
+          t (State f Sskip k e (Maps.PTree.set id v le) m).
+Proof.
+  intros. exploit deref_loc_translated; eauto. rewrite <- H1.
+  unfold make_set. destruct (chunk_for_volatile_type (typeof a)) as [chunk|].
+(* volatile case *)
+  intros. change (Maps.PTree.set id v le) with (set_opttemp (Some id) v le). econstructor.
+  econstructor. constructor. eauto.
+  simpl. unfold sem_cast. simpl. eauto. constructor.
+  simpl. econstructor; eauto.
+(* nonvolatile case *)
+  intros [A B]. subst t0. constructor. eapply eval_Elvalue; eauto.
+Qed.
+
+Lemma step_make_assign:
+  forall a1 a2 ty m b ofs t v m' v2 e le f k,
+  Csem.assign_loc ge ty m b ofs v t m' ->
+  eval_lvalue tge e le m a1 b ofs ->
+  eval_expr tge e le m a2 v2 ->
+  sem_cast v2 (typeof a2) ty m = Some v ->
+  typeof a1 = ty ->
+  step1 tge (State f (make_assign a1 a2) k e le m)
+          t (State f Sskip k e le m').
+Proof.
+  intros. exploit assign_loc_translated; eauto. rewrite <- H3.
+  unfold make_assign. destruct (chunk_for_volatile_type (typeof a1)) as [chunk|].
+(* volatile case *)
+  intros. change le with (set_opttemp None Vundef le) at 2. econstructor.
+  econstructor. constructor. eauto.
+  simpl. unfold sem_cast. simpl. eauto.
+  econstructor; eauto. rewrite H3; eauto. constructor.
+  simpl. econstructor; eauto.
+(* nonvolatile case *)
+  intros [A B]. subst t0. econstructor; eauto. congruence.
+Qed.
+
+Fixpoint Kseqlist (sl: list statement) (k: cont) :=
+  match sl with
+  | nil => k
+  | s :: l => Kseq s (Kseqlist l k)
+  end.
+
+Remark Kseqlist_app:
+  forall sl1 sl2 k,
+  Kseqlist (sl1 ++ sl2) k = Kseqlist sl1 (Kseqlist sl2 k).
+Proof.
+  induction sl1; simpl; congruence.
+Qed.
+
+Lemma push_seq:
+  forall f sl k e le m,
+  star step1 tge (State f (makeseq sl) k e le m)
+              E0 (State f Sskip (Kseqlist sl k) e le m).
+Proof.
+  intros. unfold makeseq. generalize Sskip. revert sl k.
+  induction sl; simpl; intros.
+  apply star_refl.
+  eapply star_right. apply IHsl. constructor. traceEq.
+Qed.
+
+Lemma step_tr_rvalof:
+  forall ty m b ofs t v e le a sl a' f k,
+  Csem.deref_loc ge ty m b ofs t v ->
+  eval_lvalue tge e le m a b ofs ->
+  tr_rvalof ty a (sl,a') -∗
+  ⌜ typeof a = ty ⌝ -∗
+  ∃ le',
+    ⌜star step1 tge (State f Sskip (Kseqlist sl k) e le m)
+                 t (State f Sskip k e le' m)
+  /\ eval_expr tge e le' m a' v
+  /\ typeof a' = typeof a ⌝
+  ∗ ∀ x, (\s x -∗ False) -∗ ⌜ le'!x = le!x ⌝.
+Proof.
+Admitted.
+
+(** Matching between continuations *)
+
+Inductive match_cont : Csem.cont -> cont -> Prop :=
+  | match_Kstop:
+      match_cont Csem.Kstop Kstop
+  | match_Kseq: forall s k ts tk,
+      tr_stmt s ts ->
+      match_cont k tk ->
+      match_cont (Csem.Kseq s k) (Kseq ts tk)
+  | match_Kwhile2: forall r s k s' ts tk,
+      tr_if r Sskip Sbreak s' ->
+      tr_stmt s ts ->
+      match_cont k tk ->
+      match_cont (Csem.Kwhile2 r s k)
+                 (Kloop1 (Ssequence s' ts) Sskip tk)
+  | match_Kdowhile1: forall r s k s' ts tk,
+      tr_if r Sskip Sbreak s' ->
+      tr_stmt s ts ->
+      match_cont k tk ->
+      match_cont (Csem.Kdowhile1 r s k)
+                 (Kloop1 ts s' tk)
+  | match_Kfor3: forall r s3 s k ts3 s' ts tk,
+      tr_if r Sskip Sbreak s' ->
+      tr_stmt s3 ts3 ->
+      tr_stmt s ts ->
+      match_cont k tk ->
+      match_cont (Csem.Kfor3 r s3 s k)
+                 (Kloop1 (Ssequence s' ts) ts3 tk)
+  | match_Kfor4: forall r s3 s k ts3 s' ts tk,
+      tr_if r Sskip Sbreak s' ->
+      tr_stmt s3 ts3 ->
+      tr_stmt s ts ->
+      match_cont k tk ->
+      match_cont (Csem.Kfor4 r s3 s k)
+                 (Kloop2 (Ssequence s' ts) ts3 tk)
+  | match_Kswitch2: forall k tk,
+      match_cont k tk ->
+      match_cont (Csem.Kswitch2 k) (Kswitch tk)
+  | match_Kcall: forall f e C ty k optid tf le sl tk a dest tmps,
+      tr_function f tf ->
+      leftcontext RV RV C ->
+      (forall v m, tr_top tge e (set_opttemp optid v le) m dest (C (Csyntax.Eval v ty)) sl a tmps) ->
+      match_cont_exp dest a k tk ->
+      match_cont (Csem.Kcall f e C ty k)
+                 (Kcall optid tf e le (Kseqlist sl tk))
+(*
+  | match_Kcall_some: forall f e C ty k dst tf le sl tk a dest tmps,
+      transl_function f = Errors.OK tf ->
+      leftcontext RV RV C ->
+      (forall v m, tr_top tge e (PTree.set dst v le) m dest (C (C.Eval v ty)) sl a tmps) ->
+      match_cont_exp dest a k tk ->
+      match_cont (Csem.Kcall f e C ty k)
+                 (Kcall (Some dst) tf e le (Kseqlist sl tk))
+*)
+
+with match_cont_exp : destination -> expr -> Csem.cont -> cont -> Prop :=
+  | match_Kdo: forall k a tk,
+      match_cont k tk ->
+      match_cont_exp For_effects a (Csem.Kdo k) tk
+  | match_Kifthenelse_empty: forall a k tk,
+      match_cont k tk ->
+      match_cont_exp For_val a (Csem.Kifthenelse Csyntax.Sskip Csyntax.Sskip k) (Kseq Sskip tk)
+  | match_Kifthenelse_1: forall a s1 s2 k ts1 ts2 tk,
+      tr_stmt s1 ts1 -> tr_stmt s2 ts2 ->
+      match_cont k tk ->
+      match_cont_exp For_val a (Csem.Kifthenelse s1 s2 k) (Kseq (Sifthenelse a ts1 ts2) tk)
+  | match_Kwhile1: forall r s k s' a ts tk,
+      tr_if r Sskip Sbreak s' ->
+      tr_stmt s ts ->
+      match_cont k tk ->
+      match_cont_exp For_val a
+         (Csem.Kwhile1 r s k)
+         (Kseq (makeif a Sskip Sbreak)
+           (Kseq ts (Kloop1 (Ssequence s' ts) Sskip tk)))
+  | match_Kdowhile2: forall r s k s' a ts tk,
+      tr_if r Sskip Sbreak s' ->
+      tr_stmt s ts ->
+      match_cont k tk ->
+      match_cont_exp For_val a
+        (Csem.Kdowhile2 r s k)
+        (Kseq (makeif a Sskip Sbreak) (Kloop2 ts s' tk))
+  | match_Kfor2: forall r s3 s k s' a ts3 ts tk,
+      tr_if r Sskip Sbreak s' ->
+      tr_stmt s3 ts3 ->
+      tr_stmt s ts ->
+      match_cont k tk ->
+      match_cont_exp For_val a
+        (Csem.Kfor2 r s3 s k)
+        (Kseq (makeif a Sskip Sbreak)
+          (Kseq ts (Kloop1 (Ssequence s' ts) ts3 tk)))
+  | match_Kswitch1: forall ls k a tls tk,
+      tr_lblstmts ls tls ->
+      match_cont k tk ->
+      match_cont_exp For_val a (Csem.Kswitch1 ls k) (Kseq (Sswitch a tls) tk)
+  | match_Kreturn: forall k a tk,
+      match_cont k tk ->
+      match_cont_exp For_val a (Csem.Kreturn k) (Kseq (Sreturn (Some a)) tk).
+
+Lemma match_cont_call:
+  forall k tk,
+  match_cont k tk ->
+  match_cont (Csem.call_cont k) (call_cont tk).
+Proof.
+  induction 1; simpl; auto. constructor. econstructor; eauto.
+Qed.
+
+(** Matching between states *)
+
+Inductive match_states: Csem.state -> state -> Prop :=
+  | match_exprstates: forall f r k e m tf sl tk le dest a tmps,
+      tr_function f tf ->
+      tr_top tge e le m dest r sl a tmps ->
+      match_cont_exp dest a k tk ->
+      match_states (Csem.ExprState f r k e m)
+                   (State tf Sskip (Kseqlist sl tk) e le m)
+  | match_regularstates: forall f s k e m tf ts tk le,
+      tr_function f tf ->
+      tr_stmt s ts ->
+      match_cont k tk ->
+      match_states (Csem.State f s k e m)
+                   (State tf ts tk e le m)
+  | match_callstates: forall fd args k m tfd tk,
+      tr_fundef fd tfd ->
+      match_cont k tk ->
+      match_states (Csem.Callstate fd args k m)
+                   (Callstate tfd args tk m)
+  | match_returnstates: forall res k m tk,
+      match_cont k tk ->
+      match_states (Csem.Returnstate res k m)
+                   (Returnstate res tk m)
+  | match_stuckstate: forall S,
+      match_states Csem.Stuckstate S.
+
+(** Additional results on translation of statements *)
+
+Lemma tr_select_switch:
+  forall n ls tls,
+  tr_lblstmts ls tls ->
+  tr_lblstmts (Csem.select_switch n ls) (select_switch n tls).
+Proof.
+  assert (DFL: forall ls tls,
+      tr_lblstmts ls tls ->
+      tr_lblstmts (Csem.select_switch_default ls) (select_switch_default tls)).
+  { induction 1; simpl. constructor. destruct c; auto. constructor; auto. }
+  assert (CASE: forall n ls tls,
+      tr_lblstmts ls tls ->
+      match Csem.select_switch_case n ls with
+      | None =>
+          select_switch_case n tls = None
+      | Some ls' =>
+          exists tls', select_switch_case n tls = Some tls' /\ tr_lblstmts ls' tls'
+      end).
+  { induction 1; simpl; intros.
+    auto.
+    destruct c; auto. destruct (zeq z n); auto.
+    econstructor; split; eauto. constructor; auto. }
+  intros. unfold Csem.select_switch, select_switch.
+  specialize (CASE n ls tls H).
+  destruct (Csem.select_switch_case n ls) as [ls'|].
+  destruct CASE as [tls' [P Q]]. rewrite P. auto.
+  rewrite CASE. apply DFL; auto.
+Qed.
+
+Lemma tr_seq_of_labeled_statement:
+  forall ls tls,
+  tr_lblstmts ls tls ->
+  tr_stmt (Csem.seq_of_labeled_statement ls) (seq_of_labeled_statement tls).
+Proof.
+  induction 1; simpl; constructor; auto.
+Qed.
+
+(** Commutation between translation and the "find label" operation. *)
+
+Section FIND_LABEL.
+
+Variable lbl: label.
+
+Definition nolabel (s: statement) : Prop :=
+  forall k, find_label lbl s k = None.
+
+Fixpoint nolabel_list (sl: list statement) : Prop :=
+  match sl with
+  | nil => True
+  | s1 :: sl' => nolabel s1 /\ nolabel_list sl'
+  end.
+
+Lemma nolabel_list_app:
+  forall sl2 sl1, nolabel_list sl1 -> nolabel_list sl2 -> nolabel_list (sl1 ++ sl2).
+Proof.
+  induction sl1; simpl; intros. auto. tauto.
+Qed.
+
+Lemma makeseq_nolabel:
+  forall sl, nolabel_list sl -> nolabel (makeseq sl).
+Proof.
+  assert (forall sl s, nolabel s -> nolabel_list sl -> nolabel (makeseq_rec s sl)).
+  induction sl; simpl; intros. auto. destruct H0. apply IHsl; auto.
+  red. intros; simpl. rewrite H. apply H0.
+  intros. unfold makeseq. apply H; auto. red. auto.
+Qed.
+
+Lemma makeif_nolabel:
+  forall a s1 s2, nolabel s1 -> nolabel s2 -> nolabel (makeif a s1 s2).
+Proof.
+  intros. functional induction (makeif a s1 s2); auto.
+  red; simpl; intros. rewrite H; auto.
+  red; simpl; intros. rewrite H; auto.
+Qed.
+
+Lemma make_set_nolabel:
+  forall t a, nolabel (make_set t a).
+Proof.
+  unfold make_set; intros; red; intros.
+  destruct (chunk_for_volatile_type (typeof a)); auto.
+Qed.
+
+Lemma make_assign_nolabel:
+  forall l r, nolabel (make_assign l r).
+Proof.
+  unfold make_assign; intros; red; intros.
+  destruct (chunk_for_volatile_type (typeof l)); auto.
+Qed.
+
+Lemma tr_rvalof_nolabel:
+  forall ty a sl a' tmp, tr_rvalof ty a sl a' tmp -> nolabel_list sl.
+Proof.
+  destruct 1; simpl; intuition. apply make_set_nolabel.
+Qed.
+
+Lemma nolabel_do_set:
+  forall sd a, nolabel_list (do_set sd a).
+Proof.
+  induction sd; intros; simpl; split; auto; red; auto.
+Qed.
+
+Lemma nolabel_final:
+  forall dst a, nolabel_list (final dst a).
+Proof.
+  destruct dst; simpl; intros. auto. auto. apply nolabel_do_set.
+Qed.
+
+Ltac NoLabelTac :=
+  match goal with
+  | [ |- nolabel_list nil ] => exact I
+  | [ |- nolabel_list (final _ _) ] => apply nolabel_final (*; NoLabelTac*)
+  | [ |- nolabel_list (_ :: _) ] => simpl; split; NoLabelTac
+  | [ |- nolabel_list (_ ++ _) ] => apply nolabel_list_app; NoLabelTac
+  | [ H: _ -> nolabel_list ?x |- nolabel_list ?x ] => apply H; NoLabelTac
+  | [ |- nolabel (makeseq _) ] => apply makeseq_nolabel; NoLabelTac
+  | [ |- nolabel (makeif _ _ _) ] => apply makeif_nolabel; NoLabelTac
+  | [ |- nolabel (make_set _ _) ] => apply make_set_nolabel
+  | [ |- nolabel (make_assign _ _) ] => apply make_assign_nolabel
+  | [ |- nolabel _ ] => red; intros; simpl; auto
+  | [ |- _ /\ _ ] => split; NoLabelTac
+  | _ => auto
+  end.
+
+Lemma tr_find_label_expr:
+  (forall le dst r sl a tmps, tr_expr le dst r sl a tmps -> nolabel_list sl)
+/\(forall le rl sl al tmps, tr_exprlist le rl sl al tmps -> nolabel_list sl).
+Proof.
+  apply tr_expr_exprlist; intros; NoLabelTac.
+  apply nolabel_do_set.
+  eapply tr_rvalof_nolabel; eauto.
+  apply nolabel_do_set.
+  apply nolabel_do_set.
+  eapply tr_rvalof_nolabel; eauto.
+  eapply tr_rvalof_nolabel; eauto.
+  eapply tr_rvalof_nolabel; eauto.
+Qed.
+
+Lemma tr_find_label_top:
+  forall e le m dst r sl a tmps,
+  tr_top tge e le m dst r sl a tmps -> nolabel_list sl.
+Proof.
+  induction 1; intros; NoLabelTac.
+  eapply (proj1 tr_find_label_expr); eauto.
+Qed.
+
+Lemma tr_find_label_expression:
+  forall r s a, tr_expression r s a -> forall k, find_label lbl s k = None.
+Proof.
+  intros. inv H.
+  assert (nolabel (makeseq sl)). apply makeseq_nolabel.
+  eapply tr_find_label_top with (e := empty_env) (le := PTree.empty val) (m := Mem.empty).
+  eauto. apply H.
+Qed.
+
+Lemma tr_find_label_expr_stmt:
+  forall r s, tr_expr_stmt r s -> forall k, find_label lbl s k = None.
+Proof.
+  intros. inv H.
+  assert (nolabel (makeseq sl)). apply makeseq_nolabel.
+  eapply tr_find_label_top with (e := empty_env) (le := PTree.empty val) (m := Mem.empty).
+  eauto. apply H.
+Qed.
+
+Lemma tr_find_label_if:
+  forall r s,
+  tr_if r Sskip Sbreak s ->
+  forall k, find_label lbl s k = None.
+Proof.
+  intros. inv H.
+  assert (nolabel (makeseq (sl ++ makeif a Sskip Sbreak :: nil))).
+  apply makeseq_nolabel.
+  apply nolabel_list_app.
+  eapply tr_find_label_top with (e := empty_env) (le := PTree.empty val) (m := Mem.empty).
+  eauto.
+  simpl; split; auto. apply makeif_nolabel. red; simpl; auto. red; simpl; auto.
+  apply H.
+Qed.
+
+Lemma tr_find_label:
+  forall s k ts tk
+    (TR: tr_stmt s ts)
+    (MC: match_cont k tk),
+  match Csem.find_label lbl s k with
+  | None =>
+      find_label lbl ts tk = None
+  | Some (s', k') =>
+      exists ts', exists tk',
+          find_label lbl ts tk = Some (ts', tk')
+       /\ tr_stmt s' ts'
+       /\ match_cont k' tk'
+  end
+with tr_find_label_ls:
+  forall s k ts tk
+    (TR: tr_lblstmts s ts)
+    (MC: match_cont k tk),
+  match Csem.find_label_ls lbl s k with
+  | None =>
+      find_label_ls lbl ts tk = None
+  | Some (s', k') =>
+      exists ts', exists tk',
+          find_label_ls lbl ts tk = Some (ts', tk')
+       /\ tr_stmt s' ts'
+       /\ match_cont k' tk'
+  end.
+Proof.
+  induction s; intros; inversion TR; subst; clear TR; simpl.
+  auto.
+  eapply tr_find_label_expr_stmt; eauto.
+(* seq *)
+  exploit (IHs1 (Csem.Kseq s2 k)); eauto. constructor; eauto.
+  destruct (Csem.find_label lbl s1 (Csem.Kseq s2 k)) as [[s' k'] | ].
+  intros [ts' [tk' [A [B C]]]]. rewrite A. exists ts'; exists tk'; auto.
+  intro EQ. rewrite EQ. eapply IHs2; eauto.
+(* if empty *)
+  rename s' into sr.
+  rewrite (tr_find_label_expression _ _ _ H3).
+  auto.
+(* if not empty *)
+  rename s' into sr.
+  rewrite (tr_find_label_expression _ _ _ H2).
+  exploit (IHs1 k); eauto.
+  destruct (Csem.find_label lbl s1 k) as [[s' k'] | ].
+  intros [ts' [tk' [A [B C]]]]. rewrite A. exists ts'; exists tk'; intuition.
+  intro EQ. rewrite EQ. eapply IHs2; eauto.
+(* while *)
+  rename s' into sr.
+  rewrite (tr_find_label_if _ _ H1); auto.
+  exploit (IHs (Kwhile2 e s k)); eauto. econstructor; eauto.
+  destruct (Csem.find_label lbl s (Kwhile2 e s k)) as [[s' k'] | ].
+  intros [ts' [tk' [A [B C]]]]. rewrite A. exists ts'; exists tk'; intuition.
+  intro EQ. rewrite EQ. auto.
+(* dowhile *)
+  rename s' into sr.
+  rewrite (tr_find_label_if _ _ H1); auto.
+  exploit (IHs (Kdowhile1 e s k)); eauto. econstructor; eauto.
+  destruct (Csem.find_label lbl s (Kdowhile1 e s k)) as [[s' k'] | ].
+  intros [ts' [tk' [A [B C]]]]. rewrite A. exists ts'; exists tk'; intuition.
+  intro EQ. rewrite EQ. auto.
+(* for skip *)
+  rename s' into sr.
+  rewrite (tr_find_label_if _ _ H4); auto.
+  exploit (IHs3 (Csem.Kfor3 e s2 s3 k)); eauto. econstructor; eauto.
+  destruct (Csem.find_label lbl s3 (Csem.Kfor3 e s2 s3 k)) as [[s' k'] | ].
+  intros [ts' [tk' [A [B C]]]]. rewrite A. exists ts'; exists tk'; intuition.
+  intro EQ. rewrite EQ.
+  exploit (IHs2 (Csem.Kfor4 e s2 s3 k)); eauto. econstructor; eauto.
+(* for not skip *)
+  rename s' into sr.
+  rewrite (tr_find_label_if _ _ H3); auto.
+  exploit (IHs1 (Csem.Kseq (Csyntax.Sfor Csyntax.Sskip e s2 s3) k)); eauto.
+    econstructor; eauto. econstructor; eauto.
+  destruct (Csem.find_label lbl s1
+               (Csem.Kseq (Csyntax.Sfor Csyntax.Sskip e s2 s3) k)) as [[s' k'] | ].
+  intros [ts' [tk' [A [B C]]]]. rewrite A. exists ts'; exists tk'; intuition.
+  intro EQ; rewrite EQ.
+  exploit (IHs3 (Csem.Kfor3 e s2 s3 k)); eauto. econstructor; eauto.
+  destruct (Csem.find_label lbl s3 (Csem.Kfor3 e s2 s3 k)) as [[s'' k''] | ].
+  intros [ts' [tk' [A [B C]]]]. rewrite A. exists ts'; exists tk'; intuition.
+  intro EQ'. rewrite EQ'.
+  exploit (IHs2 (Csem.Kfor4 e s2 s3 k)); eauto. econstructor; eauto.
+(* break, continue, return 0 *)
+  auto. auto. auto.
+(* return 1 *)
+  rewrite (tr_find_label_expression _ _ _ H0). auto.
+(* switch *)
+  rewrite (tr_find_label_expression _ _ _ H1). apply tr_find_label_ls. auto. constructor; auto.
+(* labeled stmt *)
+  destruct (ident_eq lbl l). exists ts0; exists tk; auto. apply IHs; auto.
+(* goto *)
+  auto.
+
+  induction s; intros; inversion TR; subst; clear TR; simpl.
+(* nil *)
+  auto.
+(* case *)
+  exploit (tr_find_label s (Csem.Kseq (Csem.seq_of_labeled_statement s0) k)); eauto.
+  econstructor; eauto. apply tr_seq_of_labeled_statement; eauto.
+  destruct (Csem.find_label lbl s
+    (Csem.Kseq (Csem.seq_of_labeled_statement s0) k)) as [[s' k'] | ].
+  intros [ts' [tk' [A [B C]]]]. rewrite A. exists ts'; exists tk'; auto.
+  intro EQ. rewrite EQ. eapply IHs; eauto.
+Qed.
+
+End FIND_LABEL.
+
+(** Anti-stuttering measure *)
+
+(** There are some stuttering steps in the translation:
+- The execution of [Sdo a] where [a] is side-effect free,
+  which is three transitions in the source:
+<<
+    Sdo a, k  --->  a, Kdo k ---> rval v, Kdo k ---> Sskip, k
+>>
+  but the translation, which is [Sskip], makes no transitions.
+- The reduction [Ecomma (Eval v) r2 --> r2].
+- The reduction [Eparen (Eval v) --> Eval v] in a [For_effects] context.
+
+The following measure decreases for these stuttering steps. *)
+
+Fixpoint esize (a: Csyntax.expr) : nat :=
+  match a with
+  | Csyntax.Eloc _ _ _ => 1%nat
+  | Csyntax.Evar _ _ => 1%nat
+  | Csyntax.Ederef r1 _ => S(esize r1)
+  | Csyntax.Efield l1 _ _ => S(esize l1)
+  | Csyntax.Eval _ _ => O
+  | Csyntax.Evalof l1 _ => S(esize l1)
+  | Csyntax.Eaddrof l1 _ => S(esize l1)
+  | Csyntax.Eunop _ r1 _ => S(esize r1)
+  | Csyntax.Ebinop _ r1 r2 _ => S(esize r1 + esize r2)%nat
+  | Csyntax.Ecast r1 _ => S(esize r1)
+  | Csyntax.Eseqand r1 _ _ => S(esize r1)
+  | Csyntax.Eseqor r1 _ _ => S(esize r1)
+  | Csyntax.Econdition r1 _ _ _ => S(esize r1)
+  | Csyntax.Esizeof _ _ => 1%nat
+  | Csyntax.Ealignof _ _ => 1%nat
+  | Csyntax.Eassign l1 r2 _ => S(esize l1 + esize r2)%nat
+  | Csyntax.Eassignop _ l1 r2 _ _ => S(esize l1 + esize r2)%nat
+  | Csyntax.Epostincr _ l1 _ => S(esize l1)
+  | Csyntax.Ecomma r1 r2 _ => S(esize r1 + esize r2)%nat
+  | Csyntax.Ecall r1 rl2 _ => S(esize r1 + esizelist rl2)%nat
+  | Csyntax.Ebuiltin ef _ rl _ => S(esizelist rl)%nat
+  | Csyntax.Eparen r1 _ _ => S(esize r1)
+  end
+
+with esizelist (el: Csyntax.exprlist) : nat :=
+  match el with
+  | Csyntax.Enil => O
+  | Csyntax.Econs r1 rl2 => (esize r1 + esizelist rl2)%nat
+  end.
+
+Definition measure (st: Csem.state) : nat :=
+  match st with
+  | Csem.ExprState _ r _ _ _ => (esize r + 1)%nat
+  | Csem.State _ Csyntax.Sskip _ _ _ => 0%nat
+  | Csem.State _ (Csyntax.Sdo r) _ _ _ => (esize r + 2)%nat
+  | Csem.State _ (Csyntax.Sifthenelse r _ _) _ _ _ => (esize r + 2)%nat
+  | _ => 0%nat
+  end.
+
+Lemma leftcontext_size:
+  forall from to C,
+  leftcontext from to C ->
+  forall e1 e2,
+  (esize e1 < esize e2)%nat ->
+  (esize (C e1) < esize (C e2))%nat
+with leftcontextlist_size:
+  forall from C,
+  leftcontextlist from C ->
+  forall e1 e2,
+  (esize e1 < esize e2)%nat ->
+  (esizelist (C e1) < esizelist (C e2))%nat.
+Proof.
+  induction 1; intros; simpl; auto with arith.
+  exploit leftcontextlist_size; eauto. auto with arith.
+  exploit leftcontextlist_size; eauto. auto with arith.
+  induction 1; intros; simpl; auto with arith. exploit leftcontext_size; eauto. auto with arith.
+Qed.
+
+(** Forward simulation for expressions. *)
+
+Lemma tr_val_gen:
+  forall le dst v ty a tmp,
+  typeof a = ty ->
+  (forall tge e le' m,
+      (forall id, In id tmp -> le'!id = le!id) ->
+      eval_expr tge e le' m a v) ->
+  tr_expr le dst (Csyntax.Eval v ty) (final dst a) a tmp.
+Proof.
+  intros. destruct dst; simpl; econstructor; auto.
+Qed.
+
+Lemma estep_simulation:
+  forall S1 t S2, Cstrategy.estep ge S1 t S2 ->
+  forall S1' (MS: match_states S1 S1'),
+  exists S2',
+     (plus step1 tge S1' t S2' \/
+       (star step1 tge S1' t S2' /\ measure S2 < measure S1)%nat)
+  /\ match_states S2 S2'.
+Proof.
+  induction 1; intros; inv MS.
+(* expr *)
+  assert (tr_expr le dest r sl a tmps).
+    inv H9. contradiction. auto.
+  exploit tr_simple_rvalue; eauto. destruct dest.
+  (* for val *)
+  intros [SL1 [TY1 EV1]]. subst sl.
+  econstructor; split.
+  right; split. apply star_refl. destruct r; simpl; (contradiction || omega).
+  econstructor; eauto.
+  instantiate (1 := tmps). apply tr_top_val_val; auto.
+  (* for effects *)
+  intros SL1. subst sl.
+  econstructor; split.
+  right; split. apply star_refl. destruct r; simpl; (contradiction || omega).
+  econstructor; eauto.
+  instantiate (1 := tmps). apply tr_top_base. constructor.
+  (* for set *)
+  inv H10.
+(* rval volatile *)
+  exploit tr_top_leftcontext; eauto. clear H11.
+  intros [dst' [sl1 [sl2 [a' [tmp' [P [Q [R S]]]]]]]].
+  inv P. inv H2. inv H7; try congruence.
+  exploit tr_simple_lvalue; eauto. intros [SL [TY EV]]. subst sl0; simpl.
+  econstructor; split.
+  left. eapply plus_two. constructor. eapply step_make_set; eauto. traceEq.
+  econstructor; eauto.
+  change (final dst' (Etempvar t0 (Csyntax.typeof l)) ++ sl2) with (nil ++ (final dst' (Etempvar t0 (Csyntax.typeof l)) ++ sl2)).
+  apply S. apply tr_val_gen. auto.
+  intros. constructor. rewrite H5; auto. apply PTree.gss.
+  intros. apply PTree.gso. red; intros; subst; elim H5; auto.
+  auto.
+(* seqand true *)
+  exploit tr_top_leftcontext; eauto. clear H9.
+  intros [dst' [sl1 [sl2 [a' [tmp' [P [Q [R S]]]]]]]].
+  inv P. inv H2.
+  (* for val *)
+  exploit tr_simple_rvalue; eauto. intros [SL [TY EV]].
+  subst sl0; simpl Kseqlist.
+  econstructor; split.
+  left. eapply plus_left. constructor.
+  eapply star_trans. apply step_makeif with (b := true) (v1 := v); auto. congruence.
+  apply push_seq. reflexivity. reflexivity.
+  rewrite <- Kseqlist_app.
+  eapply match_exprstates; eauto.
+  apply S. apply tr_paren_val with (a1 := a2); auto.
+  apply tr_expr_monotone with tmp2; eauto. auto. auto.
+  (* for effects *)
+  exploit tr_simple_rvalue; eauto. intros [SL [TY EV]].
+  subst sl0; simpl Kseqlist.
+  econstructor; split.
+  left. eapply plus_left. constructor.
+  eapply star_trans. apply step_makeif with (b := true) (v1 := v); auto. congruence.
+  apply push_seq. reflexivity. reflexivity.
+  rewrite <- Kseqlist_app.
+  eapply match_exprstates; eauto.
+  apply S. apply tr_paren_effects with (a1 := a2); auto.
+  apply tr_expr_monotone with tmp2; eauto. auto. auto.
+  (* for set *)
+  exploit tr_simple_rvalue; eauto. intros [SL [TY EV]].
+  subst sl0; simpl Kseqlist.
+  econstructor; split.
+  left. eapply plus_left. constructor.
+  eapply star_trans. apply step_makeif with (b := true) (v1 := v); auto. congruence.
+  apply push_seq. reflexivity. reflexivity.
+  rewrite <- Kseqlist_app.
+  eapply match_exprstates; eauto.
+  apply S. apply tr_paren_set with (a1 := a2) (t := sd_temp sd); auto.
+  apply tr_expr_monotone with tmp2; eauto. auto. auto.
+(* seqand false *)
+  exploit tr_top_leftcontext; eauto. clear H9.
+  intros [dst' [sl1 [sl2 [a' [tmp' [P [Q [R S]]]]]]]].
+  inv P. inv H2.
+  (* for val *)
+  exploit tr_simple_rvalue; eauto. intros [SL [TY EV]].
+  subst sl0; simpl Kseqlist.
+  econstructor; split.
+  left. eapply plus_left. constructor.
+  eapply star_trans. apply step_makeif with (b := false) (v1 := v); auto. congruence.
+  apply star_one. constructor. constructor. reflexivity. reflexivity.
+  eapply match_exprstates; eauto.
+  change sl2 with (nil ++ sl2). apply S. econstructor; eauto.
+  intros. constructor. rewrite H2. apply PTree.gss. auto.
+  intros. apply PTree.gso. congruence.
+  auto.
+  (* for effects *)
+  exploit tr_simple_rvalue; eauto. intros [SL [TY EV]].
+  subst sl0; simpl Kseqlist.
+  econstructor; split.
+  left. eapply plus_left. constructor.
+  apply step_makeif with (b := false) (v1 := v); auto. congruence.
+  reflexivity.
+  eapply match_exprstates; eauto.
+  change sl2 with (nil ++ sl2). apply S. econstructor; eauto.
+  auto. auto.
+  (* for set *)
+  exploit tr_simple_rvalue; eauto. intros [SL [TY EV]].
+  subst sl0; simpl Kseqlist.
+  econstructor; split.
+  left. eapply plus_left. constructor.
+  eapply star_trans. apply step_makeif with (b := false) (v1 := v); auto. congruence.
+  apply push_seq. reflexivity. reflexivity.
+  rewrite <- Kseqlist_app.
+  eapply match_exprstates; eauto.
+  apply S. econstructor; eauto. intros. constructor. auto. auto.
+(* seqor true *)
+  exploit tr_top_leftcontext; eauto. clear H9.
+  intros [dst' [sl1 [sl2 [a' [tmp' [P [Q [R S]]]]]]]].
+  inv P. inv H2.
+  (* for val *)
+  exploit tr_simple_rvalue; eauto. intros [SL [TY EV]].
+  subst sl0; simpl Kseqlist.
+  econstructor; split.
+  left. eapply plus_left. constructor.
+  eapply star_trans. apply step_makeif with (b := true) (v1 := v); auto. congruence.
+  apply star_one. constructor. constructor. reflexivity. reflexivity.
+  eapply match_exprstates; eauto.
+  change sl2 with (nil ++ sl2). apply S. econstructor; eauto.
+  intros. constructor. rewrite H2. apply PTree.gss. auto.
+  intros. apply PTree.gso. congruence.
+  auto.
+  (* for effects *)
+  exploit tr_simple_rvalue; eauto. intros [SL [TY EV]].
+  subst sl0; simpl Kseqlist.
+  econstructor; split.
+  left. eapply plus_left. constructor.
+  apply step_makeif with (b := true) (v1 := v); auto. congruence.
+  reflexivity.
+  eapply match_exprstates; eauto.
+  change sl2 with (nil ++ sl2). apply S. econstructor; eauto.
+  auto. auto.
+  (* for set *)
+  exploit tr_simple_rvalue; eauto. intros [SL [TY EV]].
+  subst sl0; simpl Kseqlist.
+  econstructor; split.
+  left. eapply plus_left. constructor.
+  eapply star_trans. apply step_makeif with (b := true) (v1 := v); auto. congruence.
+  apply push_seq. reflexivity. reflexivity.
+  rewrite <- Kseqlist_app.
+  eapply match_exprstates; eauto.
+  apply S. econstructor; eauto. intros. constructor. auto. auto.
+(* seqand false *)
+  exploit tr_top_leftcontext; eauto. clear H9.
+  intros [dst' [sl1 [sl2 [a' [tmp' [P [Q [R S]]]]]]]].
+  inv P. inv H2.
+  (* for val *)
+  exploit tr_simple_rvalue; eauto. intros [SL [TY EV]].
+  subst sl0; simpl Kseqlist.
+  econstructor; split.
+  left. eapply plus_left. constructor.
+  eapply star_trans. apply step_makeif with (b := false) (v1 := v); auto. congruence.
+  apply push_seq. reflexivity. reflexivity.
+  rewrite <- Kseqlist_app.
+  eapply match_exprstates; eauto.
+  apply S. apply tr_paren_val with (a1 := a2); auto.
+  apply tr_expr_monotone with tmp2; eauto. auto. auto.
+  (* for effects *)
+  exploit tr_simple_rvalue; eauto. intros [SL [TY EV]].
+  subst sl0; simpl Kseqlist.
+  econstructor; split.
+  left. eapply plus_left. constructor.
+  eapply star_trans. apply step_makeif with (b := false) (v1 := v); auto. congruence.
+  apply push_seq. reflexivity. reflexivity.
+  rewrite <- Kseqlist_app.
+  eapply match_exprstates; eauto.
+  apply S. apply tr_paren_effects with (a1 := a2); auto.
+  apply tr_expr_monotone with tmp2; eauto. auto. auto.
+  (* for set *)
+  exploit tr_simple_rvalue; eauto. intros [SL [TY EV]].
+  subst sl0; simpl Kseqlist.
+  econstructor; split.
+  left. eapply plus_left. constructor.
+  eapply star_trans. apply step_makeif with (b := false) (v1 := v); auto. congruence.
+  apply push_seq. reflexivity. reflexivity.
+  rewrite <- Kseqlist_app.
+  eapply match_exprstates; eauto.
+  apply S. apply tr_paren_set with (a1 := a2) (t := sd_temp sd); auto.
+  apply tr_expr_monotone with tmp2; eauto. auto. auto.
+(* condition *)
+  exploit tr_top_leftcontext; eauto. clear H9.
+  intros [dst' [sl1 [sl2 [a' [tmp' [P [Q [R S]]]]]]]].
+  inv P. inv H2.
+  (* for value *)
+  exploit tr_simple_rvalue; eauto. intros [SL [TY EV]].
+  subst sl0; simpl Kseqlist. destruct b.
+  econstructor; split.
+  left. eapply plus_left. constructor.
+  eapply star_trans. apply step_makeif with (b := true) (v1 := v); auto. congruence.
+  apply push_seq. reflexivity. reflexivity.
+  rewrite <- Kseqlist_app.
+  eapply match_exprstates; eauto.
+  apply S. econstructor; eauto. apply tr_expr_monotone with tmp2; eauto. auto. auto.
+  econstructor; split.
+  left. eapply plus_left. constructor.
+  eapply star_trans. apply step_makeif with (b := false) (v1 := v); auto. congruence.
+  apply push_seq. reflexivity. reflexivity.
+  rewrite <- Kseqlist_app.
+  eapply match_exprstates; eauto.
+  apply S. econstructor; eauto. apply tr_expr_monotone with tmp3; eauto. auto. auto.
+  (* for effects *)
+  exploit tr_simple_rvalue; eauto. intros [SL [TY EV]].
+  subst sl0; simpl Kseqlist. destruct b.
+  econstructor; split.
+  left. eapply plus_left. constructor.
+  eapply star_trans. apply step_makeif with (b := true) (v1 := v); auto. congruence.
+  apply push_seq.
+  reflexivity. traceEq.
+  rewrite <- Kseqlist_app.
+  econstructor. eauto. apply S.
+    econstructor; eauto. apply tr_expr_monotone with tmp2; eauto.
+    econstructor; eauto.
+  auto. auto.
+  econstructor; split.
+  left. eapply plus_left. constructor.
+  eapply star_trans. apply step_makeif with (b := false) (v1 := v); auto. congruence.
+  apply push_seq.
+  reflexivity. traceEq.
+  rewrite <- Kseqlist_app.
+  econstructor. eauto. apply S.
+    econstructor; eauto. apply tr_expr_monotone with tmp3; eauto.
+    econstructor; eauto.
+  auto. auto.
+  (* for set *)
+  exploit tr_simple_rvalue; eauto. intros [SL [TY EV]].
+  subst sl0; simpl Kseqlist. destruct b.
+  econstructor; split.
+  left. eapply plus_left. constructor.
+  eapply star_trans. apply step_makeif with (b := true) (v1 := v); auto. congruence.
+  apply push_seq.
+  reflexivity. traceEq.
+  rewrite <- Kseqlist_app.
+  econstructor. eauto. apply S.
+    econstructor; eauto. apply tr_expr_monotone with tmp2; eauto.
+    econstructor; eauto.
+  auto. auto.
+  econstructor; split.
+  left. eapply plus_left. constructor.
+  eapply star_trans. apply step_makeif with (b := false) (v1 := v); auto. congruence.
+  apply push_seq.
+  reflexivity. traceEq.
+  rewrite <- Kseqlist_app.
+  econstructor. eauto. apply S.
+    econstructor; eauto. apply tr_expr_monotone with tmp3; eauto.
+    econstructor; eauto.
+  auto. auto.
+(* assign *)
+  exploit tr_top_leftcontext; eauto. clear H12.
+  intros [dst' [sl1 [sl2 [a' [tmp' [P [Q [R S]]]]]]]].
+  inv P. inv H4.
+  (* for effects *)
+  exploit tr_simple_rvalue; eauto. intros [SL2 [TY2 EV2]].
+  exploit tr_simple_lvalue; eauto. intros [SL1 [TY1 EV1]].
+  subst; simpl Kseqlist.
+  econstructor; split.
+  left. eapply plus_left. constructor.
+  apply star_one. eapply step_make_assign; eauto.
+  rewrite <- TY2; eauto. traceEq.
+  econstructor. auto. change sl2 with (nil ++ sl2). apply S.
+  constructor. auto. auto. auto.
+  (* for value *)
+  exploit tr_simple_rvalue; eauto. intros [SL2 [TY2 EV2]].
+  exploit tr_simple_lvalue. eauto.
+    eapply tr_expr_invariant with (le' := PTree.set t0 v' le). eauto.
+    intros. apply PTree.gso. intuition congruence.
+  intros [SL1 [TY1 EV1]].
+  subst; simpl Kseqlist.
+  econstructor; split.
+  left. eapply plus_left. constructor.
+  eapply star_left. constructor. econstructor. eauto. rewrite <- TY2; eauto. 
+  eapply star_left. constructor.
+  apply star_one. eapply step_make_assign; eauto.
+  constructor. apply PTree.gss. simpl. eapply cast_idempotent; eauto. 
+  reflexivity. reflexivity. traceEq.
+  econstructor. auto. apply S.
+  apply tr_val_gen. auto. intros. constructor.
+  rewrite H4; auto. apply PTree.gss.
+  intros. apply PTree.gso. intuition congruence.
+  auto. auto.
+(* assignop *)
+  exploit tr_top_leftcontext; eauto. clear H15.
+  intros [dst' [sl1 [sl2 [a' [tmp' [P [Q [R S]]]]]]]].
+  inv P. inv H6.
+  (* for effects *)
+  exploit tr_simple_lvalue; eauto. intros [SL1 [TY1 EV1]].
+  exploit step_tr_rvalof; eauto. intros [le' [EXEC [EV3 [TY3 INV]]]].
+  exploit tr_simple_lvalue. eauto. eapply tr_expr_invariant with (le := le) (le' := le'). eauto.
+  intros. apply INV. NOTIN. intros [? [? EV1']].
+  exploit tr_simple_rvalue. eauto. eapply tr_expr_invariant with (le := le) (le' := le'). eauto.
+  intros. apply INV. NOTIN. simpl. intros [SL2 [TY2 EV2]].
+  subst; simpl Kseqlist.
+  econstructor; split.
+  left. eapply star_plus_trans. rewrite app_ass. rewrite Kseqlist_app. eexact EXEC.
+  eapply plus_two. simpl. econstructor. eapply step_make_assign; eauto.
+    econstructor. eexact EV3. eexact EV2.
+    rewrite TY3; rewrite <- TY1; rewrite <- TY2; rewrite comp_env_preserved; auto.
+  reflexivity. traceEq.
+  econstructor. auto. change sl2 with (nil ++ sl2). apply S.
+  constructor. auto. auto. auto.
+  (* for value *)
+  exploit tr_simple_lvalue; eauto. intros [SL1 [TY1 EV1]].
+  exploit step_tr_rvalof; eauto. intros [le' [EXEC [EV3 [TY3 INV]]]].
+  exploit tr_simple_lvalue. eauto. eapply tr_expr_invariant with (le := le) (le' := le'). eauto.
+  intros. apply INV. NOTIN. intros [? [? EV1']].
+  exploit tr_simple_rvalue. eauto. eapply tr_expr_invariant with (le := le) (le' := le'). eauto.
+  intros. apply INV. NOTIN. simpl. intros [SL2 [TY2 EV2]].
+  exploit tr_simple_lvalue. eauto.
+    eapply tr_expr_invariant with (le := le) (le' := PTree.set t v4 le'). eauto.
+    intros. rewrite PTree.gso. apply INV. NOTIN. intuition congruence.
+  intros [? [? EV1'']].
+  subst; simpl Kseqlist.
+  econstructor; split.
+  left. rewrite app_ass. rewrite Kseqlist_app.
+  eapply star_plus_trans. eexact EXEC.
+  simpl. eapply plus_four. econstructor. econstructor.
+    econstructor. econstructor. eexact EV3. eexact EV2.
+    rewrite TY3; rewrite <- TY1; rewrite <- TY2; rewrite comp_env_preserved; eauto.
+    eassumption.
+  econstructor. eapply step_make_assign; eauto.
+    constructor. apply PTree.gss. simpl. eapply cast_idempotent; eauto.
+    reflexivity. traceEq.
+  econstructor. auto. apply S.
+  apply tr_val_gen. auto. intros. constructor.
+  rewrite H10; auto. apply PTree.gss.
+  intros. rewrite PTree.gso. apply INV.
+  red; intros; elim H10; auto.
+  intuition congruence.
+  auto. auto.
+(* assignop stuck *)
+  exploit tr_top_leftcontext; eauto. clear H12.
+  intros [dst' [sl1 [sl2 [a' [tmp' [P [Q [R S]]]]]]]].
+  inv P. inv H4.
+  (* for effects *)
+  exploit tr_simple_lvalue; eauto. intros [SL1 [TY1 EV1]].
+  exploit tr_simple_rvalue; eauto. intros [SL2 [TY2 EV2]].
+  exploit step_tr_rvalof; eauto. intros [le' [EXEC [EV3 [TY3 INV]]]].
+  subst; simpl Kseqlist.
+  econstructor; split.
+  right; split. rewrite app_ass. rewrite Kseqlist_app. eexact EXEC.
+  simpl. omega.
+  constructor.
+  (* for value *)
+  exploit tr_simple_lvalue; eauto. intros [SL1 [TY1 EV1]].
+  exploit tr_simple_rvalue; eauto. intros [SL2 [TY2 EV2]].
+  exploit step_tr_rvalof; eauto. intros [le' [EXEC [EV3 [TY3 INV]]]].
+  subst; simpl Kseqlist.
+  econstructor; split.
+  right; split. rewrite app_ass. rewrite Kseqlist_app. eexact EXEC.
+  simpl. omega.
+  constructor.
+(* postincr *)
+  exploit tr_top_leftcontext; eauto. clear H14.
+  intros [dst' [sl1 [sl2 [a' [tmp' [P [Q [R S]]]]]]]].
+  inv P. inv H5.
+  (* for effects *)
+  exploit tr_simple_lvalue; eauto. intros [SL1 [TY1 EV1]].
+  exploit step_tr_rvalof; eauto. intros [le' [EXEC [EV3 [TY3 INV]]]].
+  exploit tr_simple_lvalue. eauto. eapply tr_expr_invariant with (le := le) (le' := le'). eauto.
+  intros. apply INV. NOTIN. intros [? [? EV1']].
+  subst; simpl Kseqlist.
+  econstructor; split.
+  left. rewrite app_ass; rewrite Kseqlist_app.
+  eapply star_plus_trans. eexact EXEC.
+  eapply plus_two. simpl. constructor.
+  eapply step_make_assign; eauto.
+  unfold transl_incrdecr. destruct id; simpl in H2.
+  econstructor. eauto. constructor. rewrite TY3; rewrite <- TY1; rewrite comp_env_preserved. simpl; eauto.
+  econstructor. eauto. constructor. rewrite TY3; rewrite <- TY1; rewrite comp_env_preserved. simpl; eauto.
+  destruct id; auto.
+  reflexivity. traceEq.
+  econstructor. auto. change sl2 with (nil ++ sl2). apply S.
+  constructor. auto. auto. auto.
+  (* for value *)
+  exploit tr_simple_lvalue; eauto. intros [SL1 [TY1 EV1]].
+  exploit tr_simple_lvalue. eauto.
+    eapply tr_expr_invariant with (le' := PTree.set t v1 le). eauto.
+    intros. apply PTree.gso. intuition congruence.
+  intros [SL2 [TY2 EV2]].
+  subst; simpl Kseqlist.
+  econstructor; split.
+  left. eapply plus_four. constructor.
+  eapply step_make_set; eauto.
+  constructor.
+  eapply step_make_assign; eauto.
+  unfold transl_incrdecr. destruct id; simpl in H2.
+  econstructor. constructor. apply PTree.gss. constructor.
+  rewrite comp_env_preserved; simpl; eauto.
+  econstructor. constructor. apply PTree.gss. constructor.
+  rewrite comp_env_preserved; simpl; eauto.
+  destruct id; auto.
+  traceEq.
+  econstructor. auto. apply S.
+  apply tr_val_gen. auto. intros. econstructor; eauto.
+  rewrite H5; auto. apply PTree.gss.
+  intros. apply PTree.gso. intuition congruence.
+  auto. auto.
+(* postincr stuck *)
+  exploit tr_top_leftcontext; eauto. clear H11.
+  intros [dst' [sl1 [sl2 [a' [tmp' [P [Q [R S]]]]]]]].
+  inv P. inv H3.
+  (* for effects *)
+  exploit tr_simple_lvalue; eauto. intros [SL1 [TY1 EV1]].
+  exploit step_tr_rvalof; eauto. intros [le' [EXEC [EV3 [TY3 INV]]]].
+  subst. simpl Kseqlist.
+  econstructor; split.
+  right; split. rewrite app_ass; rewrite Kseqlist_app. eexact EXEC.
+  simpl; omega.
+  constructor.
+  (* for value *)
+  exploit tr_simple_lvalue; eauto. intros [SL1 [TY1 EV1]].
+  subst. simpl Kseqlist.
+  econstructor; split.
+  left. eapply plus_two. constructor. eapply step_make_set; eauto.
+  traceEq.
+  constructor.
+(* comma *)
+  exploit tr_top_leftcontext; eauto. clear H9.
+  intros [dst' [sl1 [sl2 [a' [tmp' [P [Q [R S]]]]]]]].
+  inv P. inv H1.
+  exploit tr_simple_rvalue; eauto. simpl; intro SL1.
+  subst sl0; simpl Kseqlist.
+  econstructor; split.
+  right; split. apply star_refl. simpl. apply plus_lt_compat_r.
+  apply (leftcontext_size _ _ _ H). simpl. omega.
+  econstructor; eauto. apply S.
+  eapply tr_expr_monotone; eauto.
+  auto. auto.
+(* paren *)
+  exploit tr_top_leftcontext; eauto. clear H9.
+  intros [dst' [sl1 [sl2 [a' [tmp' [P [Q [R S]]]]]]]].
+  inv P. inv H2.
+  (* for value *)
+  exploit tr_simple_rvalue; eauto. intros [b [SL1 [TY1 EV1]]].
+  subst sl1; simpl Kseqlist.
+  econstructor; split.
+  left. eapply plus_left. constructor. apply star_one.
+  econstructor. econstructor; eauto. rewrite <- TY1; eauto. traceEq.
+  econstructor; eauto.
+  change sl2 with (final For_val (Etempvar t (Csyntax.typeof r)) ++ sl2). apply S.
+  constructor. auto. intros. constructor. rewrite H2; auto. apply PTree.gss.
+  intros. apply PTree.gso. intuition congruence.
+  auto.
+  (* for effects *)
+  econstructor; split.
+  right; split. apply star_refl. simpl. apply plus_lt_compat_r.
+  apply (leftcontext_size _ _ _ H). simpl. omega.
+  econstructor; eauto.
+  exploit tr_simple_rvalue; eauto. simpl. intros A. subst sl1.
+  apply S. constructor; auto. auto. auto.
+  (* for set *)
+  exploit tr_simple_rvalue; eauto. simpl. intros [b [SL1 [TY1 EV1]]]. subst sl1.
+  simpl Kseqlist.
+  econstructor; split.
+  left. eapply plus_left. constructor. apply star_one. econstructor. econstructor; eauto.
+  rewrite <- TY1; eauto. traceEq.
+  econstructor; eauto.
+  apply S. constructor; auto.
+  intros. constructor. rewrite H2. apply PTree.gss. auto.
+  intros. apply PTree.gso. congruence.
+  auto.
+
+(* call *)
+  exploit tr_top_leftcontext; eauto. clear H12.
+  intros [dst' [sl1 [sl2 [a' [tmp' [P [Q [R S]]]]]]]].
+  inv P. inv H5.
+  (* for effects *)
+  exploit tr_simple_rvalue; eauto. intros [SL1 [TY1 EV1]].
+  exploit tr_simple_exprlist; eauto. intros [SL2 EV2].
+  subst. simpl Kseqlist.
+  exploit functions_translated; eauto. intros [tfd [J K]].
+  econstructor; split.
+  left. eapply plus_left. constructor.  apply star_one.
+  econstructor; eauto. rewrite <- TY1; eauto.
+  exploit type_of_fundef_preserved; eauto. congruence.
+  traceEq.
+  constructor; auto. econstructor; eauto.
+  intros. change sl2 with (nil ++ sl2). apply S.
+  constructor. auto. auto.
+  (* for value *)
+  exploit tr_simple_rvalue; eauto. intros [SL1 [TY1 EV1]].
+  exploit tr_simple_exprlist; eauto. intros [SL2 EV2].
+  subst. simpl Kseqlist.
+  exploit functions_translated; eauto. intros [tfd [J K]].
+  econstructor; split.
+  left. eapply plus_left. constructor.  apply star_one.
+  econstructor; eauto. rewrite <- TY1; eauto.
+  exploit type_of_fundef_preserved; eauto. congruence.
+  traceEq.
+  constructor; auto. econstructor; eauto.
+  intros. apply S.
+  destruct dst'; constructor.
+  auto. intros. constructor. rewrite H5; auto. apply PTree.gss.
+  auto. intros. constructor. rewrite H5; auto. apply PTree.gss.
+  intros. apply PTree.gso. intuition congruence.
+  auto.
+
+(* builtin *)
+  exploit tr_top_leftcontext; eauto. clear H9.
+  intros [dst' [sl1 [sl2 [a' [tmp' [P [Q [R S]]]]]]]].
+  inv P. inv H2.
+  (* for effects *)
+  exploit tr_simple_exprlist; eauto. intros [SL EV].
+  subst. simpl Kseqlist.
+  econstructor; split.
+  left. eapply plus_left. constructor.  apply star_one.
+  econstructor; eauto.
+  eapply external_call_symbols_preserved; eauto. apply senv_preserved.
+  traceEq.
+  econstructor; eauto.
+  change sl2 with (nil ++ sl2). apply S. constructor. simpl; auto. auto.
+  (* for value *)
+  exploit tr_simple_exprlist; eauto. intros [SL EV].
+  subst. simpl Kseqlist.
+  econstructor; split.
+  left. eapply plus_left. constructor. apply star_one.
+  econstructor; eauto.
+  eapply external_call_symbols_preserved; eauto. apply senv_preserved.
+  traceEq.
+  econstructor; eauto.
+  change sl2 with (nil ++ sl2). apply S.
+  apply tr_val_gen. auto. intros. constructor. rewrite H2; auto. simpl. apply PTree.gss.
+  intros; simpl. apply PTree.gso. intuition congruence.
+  auto.
+Qed.
+
+(** Forward simulation for statements. *)
+
+Lemma tr_top_val_for_val_inv:
+  forall e le m v ty sl a tmps,
+  tr_top tge e le m For_val (Csyntax.Eval v ty) sl a tmps ->
+  sl = nil /\ typeof a = ty /\ eval_expr tge e le m a v.
+Proof.
+  intros. inv H. auto. inv H0. auto.
+Qed.
+
+Lemma alloc_variables_preserved:
+  forall e m params e' m',
+  Csem.alloc_variables ge e m params e' m' ->
+  alloc_variables tge e m params e' m'.
+Proof.
+  induction 1; econstructor; eauto. rewrite comp_env_preserved; auto.
+Qed.
+
+Lemma bind_parameters_preserved:
+  forall e m params args m',
+  Csem.bind_parameters ge e m params args m' ->
+  bind_parameters tge e m params args m'.
+Proof.
+  induction 1; econstructor; eauto. inv H0.
+- eapply assign_loc_value; eauto.
+- inv H4. eapply assign_loc_value; eauto.
+- rewrite <- comp_env_preserved in *. eapply assign_loc_copy; eauto.
+Qed.
+
+Lemma blocks_of_env_preserved:
+  forall e, blocks_of_env tge e = Csem.blocks_of_env ge e.
+Proof.
+  intros; unfold blocks_of_env, Csem.blocks_of_env.
+  unfold block_of_binding, Csem.block_of_binding.
+  rewrite comp_env_preserved. auto.
+Qed.
+
+Lemma sstep_simulation:
+  forall S1 t S2, Csem.sstep ge S1 t S2 ->
+  forall S1' (MS: match_states S1 S1'),
+  exists S2',
+     (plus step1 tge S1' t S2' \/
+       (star step1 tge S1' t S2' /\ measure S2 < measure S1)%nat)
+  /\ match_states S2 S2'.
+Proof.
+  induction 1; intros; inv MS.
+(* do 1 *)
+  inv H6. inv H0.
+  econstructor; split.
+  right; split. apply push_seq.
+  simpl. omega.
+  econstructor; eauto. constructor. auto.
+(* do 2 *)
+  inv H7. inv H6. inv H.
+  econstructor; split.
+  right; split. apply star_refl. simpl. omega.
+  econstructor; eauto. constructor.
+
+(* seq *)
+  inv H6. econstructor; split. left. apply plus_one. constructor.
+  econstructor; eauto. constructor; auto.
+(* skip seq *)
+  inv H6; inv H7. econstructor; split.
+  left. apply plus_one; constructor.
+  econstructor; eauto.
+(* continue seq *)
+  inv H6; inv H7. econstructor; split.
+  left. apply plus_one; constructor.
+  econstructor; eauto. constructor.
+(* break seq *)
+  inv H6; inv H7. econstructor; split.
+  left. apply plus_one; constructor.
+  econstructor; eauto. constructor.
+(* ifthenelse *)
+  inv H6.
+(* ifthenelse empty *)
+  inv H3. econstructor; split.
+  left. eapply plus_left. constructor. apply push_seq.
+  econstructor; eauto.
+  econstructor; eauto.
+  econstructor; eauto.
+(* ifthenelse non empty *)
+  inv H2. econstructor; split.
+  left. eapply plus_left. constructor. apply push_seq. traceEq.
+  econstructor; eauto. econstructor; eauto.
+(* ifthenelse *)
+  inv H8.
+(* ifthenelse empty *)
+  exploit tr_top_val_for_val_inv; eauto. intros [A [B C]]. subst.
+  econstructor; split; simpl.
+  right. destruct b; econstructor; eauto.
+  eapply star_left. apply step_skip_seq. econstructor. traceEq.
+  eapply star_left. apply step_skip_seq. econstructor. traceEq.
+  destruct b; econstructor; eauto. econstructor; eauto. econstructor; eauto.
+  (* ifthenelse non empty *)
+  exploit tr_top_val_for_val_inv; eauto. intros [A [B C]]. subst.
+  econstructor; split.
+  left. eapply plus_two. constructor.
+  apply step_ifthenelse with (v1 := v) (b := b); auto. traceEq.
+  destruct b; econstructor; eauto.
+(* while *)
+  inv H6. inv H1. econstructor; split.
+  left. eapply plus_left. constructor.
+  eapply star_left. constructor.
+  apply push_seq.
+  reflexivity. traceEq. rewrite Kseqlist_app.
+  econstructor; eauto. simpl.  econstructor; eauto. econstructor; eauto.
+(* while false *)
+  inv H8.
+  exploit tr_top_val_for_val_inv; eauto. intros [A [B C]]. subst.
+  econstructor; split.
+  left. simpl. eapply plus_left. constructor.
+  eapply star_trans. apply step_makeif with (v1 := v) (b := false); auto.
+  eapply star_two. constructor. apply step_break_loop1.
+  reflexivity. reflexivity. traceEq.
+  constructor; auto. constructor.
+(* while true *)
+  inv H8.
+  exploit tr_top_val_for_val_inv; eauto. intros [A [B C]]. subst.
+  econstructor; split.
+  left. simpl. eapply plus_left. constructor.
+  eapply star_right. apply step_makeif with (v1 := v) (b := true); auto.
+  constructor.
+  reflexivity. traceEq.
+  constructor; auto. constructor; auto.
+(* skip-or-continue while *)
+  assert (ts = Sskip \/ ts = Scontinue). destruct H; subst s0; inv H7; auto.
+  inv H8.
+  econstructor; split.
+  left. eapply plus_two. apply step_skip_or_continue_loop1; auto.
+  apply step_skip_loop2. traceEq.
+  constructor; auto. constructor; auto.
+(* break while *)
+  inv H6. inv H7.
+  econstructor; split.
+  left. apply plus_one. apply step_break_loop1.
+  constructor; auto. constructor.
+
+(* dowhile *)
+  inv H6.
+  econstructor; split.
+  left. apply plus_one. apply step_loop.
+  constructor; auto. constructor; auto.
+(* skip_or_continue dowhile *)
+  assert (ts = Sskip \/ ts = Scontinue). destruct H; subst s0; inv H7; auto.
+  inv H8. inv H4.
+  econstructor; split.
+  left. eapply plus_left. apply step_skip_or_continue_loop1. auto.
+  apply push_seq.
+  traceEq.
+  rewrite Kseqlist_app.
+  econstructor; eauto. simpl. econstructor; auto. econstructor; eauto.
+(* dowhile false *)
+  inv H8.
+  exploit tr_top_val_for_val_inv; eauto. intros [A [B C]]. subst.
+  econstructor; split.
+  left. simpl. eapply plus_left. constructor.
+  eapply star_right. apply step_makeif with (v1 := v) (b := false); auto.
+  constructor.
+  reflexivity. traceEq.
+  constructor; auto. constructor.
+(* dowhile true *)
+  inv H8.
+  exploit tr_top_val_for_val_inv; eauto. intros [A [B C]]. subst.
+  econstructor; split.
+  left. simpl. eapply plus_left. constructor.
+  eapply star_right. apply step_makeif with (v1 := v) (b := true); auto.
+  constructor.
+  reflexivity. traceEq.
+  constructor; auto. constructor; auto.
+(* break dowhile *)
+  inv H6. inv H7.
+  econstructor; split.
+  left. apply plus_one. apply step_break_loop1.
+  constructor; auto. constructor.
+
+(* for start *)
+  inv H7. congruence.
+  econstructor; split.
+  left; apply plus_one. constructor.
+  econstructor; eauto. constructor; auto. econstructor; eauto.
+(* for *)
+  inv H6; try congruence. inv H2.
+  econstructor; split.
+  left. eapply plus_left. apply step_loop.
+  eapply star_left. constructor. apply push_seq.
+  reflexivity. traceEq.
+  rewrite Kseqlist_app. econstructor; eauto. simpl. constructor; auto. econstructor; eauto.
+(* for false *)
+  inv H8. exploit tr_top_val_for_val_inv; eauto. intros [A [B C]]. subst.
+  econstructor; split.
+  left. simpl. eapply plus_left. constructor.
+  eapply star_trans. apply step_makeif with (v1 := v) (b := false); auto.
+  eapply star_two. constructor. apply step_break_loop1.
+  reflexivity. reflexivity. traceEq.
+  constructor; auto. constructor.
+(* for true *)
+  inv H8. exploit tr_top_val_for_val_inv; eauto. intros [A [B C]]. subst.
+  econstructor; split.
+  left. simpl. eapply plus_left. constructor.
+  eapply star_right. apply step_makeif with (v1 := v) (b := true); auto.
+  constructor.
+  reflexivity. traceEq.
+  constructor; auto. constructor; auto.
+(* skip_or_continue for3 *)
+  assert (ts = Sskip \/ ts = Scontinue). destruct H; subst x; inv H7; auto.
+  inv H8.
+  econstructor; split.
+  left. apply plus_one. apply step_skip_or_continue_loop1. auto.
+  econstructor; eauto. econstructor; auto.
+(* break for3 *)
+  inv H6. inv H7.
+  econstructor; split.
+  left. apply plus_one. apply step_break_loop1.
+  econstructor; eauto. constructor.
+(* skip for4 *)
+  inv H6. inv H7.
+  econstructor; split.
+  left. apply plus_one. constructor.
+  econstructor; eauto. constructor; auto.
+
+
+(* return none *)
+  inv H7. econstructor; split.
+  left. apply plus_one. econstructor; eauto. rewrite blocks_of_env_preserved; eauto.
+  constructor. apply match_cont_call; auto.
+(* return some 1 *)
+  inv H6. inv H0. econstructor; split.
+  left; eapply plus_left. constructor. apply push_seq. traceEq.
+  econstructor; eauto. constructor. auto.
+(* return some 2 *)
+  inv H9. exploit tr_top_val_for_val_inv; eauto. intros [A [B C]]. subst.
+  econstructor; split.
+  left. eapply plus_two. constructor. econstructor. eauto.
+  erewrite function_return_preserved; eauto. rewrite blocks_of_env_preserved; eauto.
+  eauto. traceEq.
+  constructor. apply match_cont_call; auto.
+(* skip return *)
+  inv H8.
+  assert (is_call_cont tk). inv H9; simpl in *; auto.
+  econstructor; split.
+  left. apply plus_one. apply step_skip_call; eauto. rewrite blocks_of_env_preserved; eauto.
+  constructor. auto.
+
+(* switch *)
+  inv H6. inv H1.
+  econstructor; split.
+  left; eapply plus_left. constructor. apply push_seq. traceEq.
+  econstructor; eauto. constructor; auto.
+(* expr switch *)
+  inv H8. exploit tr_top_val_for_val_inv; eauto. intros [A [B C]]. subst.
+  econstructor; split.
+  left; eapply plus_two. constructor. econstructor; eauto. traceEq.
+  econstructor; eauto.
+  apply tr_seq_of_labeled_statement. apply tr_select_switch. auto.
+  constructor; auto.
+
+(* skip-or-break switch *)
+  assert (ts = Sskip \/ ts = Sbreak). destruct H; subst x; inv H7; auto.
+  inv H8.
+  econstructor; split.
+  left; apply plus_one. apply step_skip_break_switch. auto.
+  constructor; auto. constructor.
+
+(* continue switch *)
+  inv H6. inv H7.
+  econstructor; split.
+  left; apply plus_one. apply step_continue_switch.
+  constructor; auto. constructor.
+
+(* label *)
+  inv H6. econstructor; split.
+  left; apply plus_one. constructor.
+  constructor; auto.
+
+(* goto *)
+  inv H7.
+  inversion H6; subst.
+  exploit tr_find_label. eauto. apply match_cont_call. eauto.
+  instantiate (1 := lbl). rewrite H.
+  intros [ts' [tk' [P [Q R]]]].
+  econstructor; split.
+  left. apply plus_one. econstructor; eauto.
+  econstructor; eauto.
+
+(* internal function *)
+  inv H7. inversion H3; subst.
+  econstructor; split.
+  left; apply plus_one. eapply step_internal_function. econstructor.
+  rewrite H6; rewrite H7; auto.
+  rewrite H6; rewrite H7. eapply alloc_variables_preserved; eauto.
+  rewrite H6. eapply bind_parameters_preserved; eauto.
+  eauto.
+  constructor; auto.
+
+(* external function *)
+  inv H5.
+  econstructor; split.
+  left; apply plus_one. econstructor; eauto.
+  eapply external_call_symbols_preserved; eauto. apply senv_preserved.
+  constructor; auto.
+
+(* return *)
+  inv H3.
+  econstructor; split.
+  left; apply plus_one. constructor.
+  econstructor; eauto.
+Qed.
+
+(** Semantic preservation *)
+
+Theorem simulation:
+  forall S1 t S2, Cstrategy.step ge S1 t S2 ->
+  forall S1' (MS: match_states S1 S1'),
+  exists S2',
+     (plus step1 tge S1' t S2' \/
+       (star step1 tge S1' t S2' /\ measure S2 < measure S1)%nat)
+  /\ match_states S2 S2'.
+Proof.
+  intros S1 t S2 STEP. destruct STEP.
+  apply estep_simulation; auto.
+  apply sstep_simulation; auto.
+Qed.
+
+Lemma transl_initial_states:
+  forall S,
+  Csem.initial_state prog S ->
+  exists S', Clight.initial_state tprog S' /\ match_states S S'.
+Proof.
+  intros. inv H.
+  exploit function_ptr_translated; eauto. intros [tf [FIND TR]].
+  econstructor; split.
+  econstructor.
+  eapply (Genv.init_mem_match (proj1 TRANSL)); eauto.
+  replace (prog_main tprog) with (prog_main prog).
+  rewrite symbols_preserved. eauto. 
+  destruct TRANSL. destruct H as (A & B & C). simpl in B. auto. 
+  eexact FIND.
+  rewrite <- H3. apply type_of_fundef_preserved. auto.
+  constructor. auto. constructor.
+Qed.
+
+Lemma transl_final_states:
+  forall S S' r,
+  match_states S S' -> Csem.final_state S r -> Clight.final_state S' r.
+Proof.
+  intros. inv H0. inv H. inv H4. constructor.
+Qed.
+
+Theorem transl_program_correct:
+  forward_simulation (Cstrategy.semantics prog) (Clight.semantics1 tprog).
+Proof.
+  eapply forward_simulation_star_wf with (order := ltof _ measure).
+  eapply senv_preserved.
+  eexact transl_initial_states.
+  eexact transl_final_states.
+  apply well_founded_ltof.
+  exact simulation.
+Qed.
+
+End PRESERVATION.
+
+(** ** Commutation with linking *)
+
+Instance TransfSimplExprLink : TransfLink match_prog.
+Proof.
+  red; intros. eapply Ctypes.link_match_program; eauto. 
+- intros.
+Local Transparent Linker_fundef.
+  simpl in *; unfold link_fundef in *. inv H3; inv H4; try discriminate.
+  destruct ef; inv H2. exists (Internal tf); split; auto. constructor; auto.
+  destruct ef; inv H2. exists (Internal tf); split; auto. constructor; auto.
+  destruct (external_function_eq ef ef0 && typelist_eq targs targs0 &&
+            type_eq tres tres0 && calling_convention_eq cconv cconv0); inv H2.
+  exists (External ef targs tres cconv); split; auto. constructor.
+Qed.
